<?xml version="1.0"?>


<!DOCTYPE rdf:RDF [
    <!ENTITY dct "http://purl.org/dc/terms/" >
    <!ENTITY prov "http://www.w3.org/ns/prov#" >
    <!ENTITY l0 "http://dati.gov.it/onto/l0/" >
    <!ENTITY owl "http://www.w3.org/2002/07/owl#" >
    <!ENTITY dc "http://purl.org/dc/elements/1.1/" >
    <!ENTITY xsd "http://www.w3.org/2001/XMLSchema#" >
    <!ENTITY rdfs "http://www.w3.org/2000/01/rdf-schema#" >
    <!ENTITY rdf "http://www.w3.org/1999/02/22-rdf-syntax-ns#" >
]>


<rdf:RDF xmlns="http://dati.gov.it/onto/cpvapit/"
     xml:base="http://dati.gov.it/onto/cpvapit/"
     xmlns:dct="http://purl.org/dc/terms/"
     xmlns:l0="http://dati.gov.it/onto/l0/"
     xmlns:rdf="http://www.w3.org/1999/02/22-rdf-syntax-ns#"
     xmlns:owl="http://www.w3.org/2002/07/owl#"
     xmlns:xsd="http://www.w3.org/2001/XMLSchema#"
     xmlns:rdfs="http://www.w3.org/2000/01/rdf-schema#"
     xmlns:prov="http://www.w3.org/ns/prov#"
     xmlns:dc="http://purl.org/dc/elements/1.1/">
    <owl:Ontology rdf:about="http://dati.gov.it/onto/cpvapit/">
        <rdfs:label xml:lang="en">Person ontology</rdfs:label>
        <rdfs:label xml:lang="it">Ontologia delle persone</rdfs:label>
        <dct:issued rdf:datatype="&xsd;date">2017-07-19</dct:issued>
        <dct:modified>2017-08-08</dct:modified>
        <dc:creator xml:lang="en">Agency for Digital Italy - AgID</dc:creator>
        <dc:creator xml:lang="en">Institute of Cognitive Sciences and Technologies of the Italian Research Council (CNR) - Semantic Technology Laboratory (STLab)</dc:creator>
        <dc:creator xml:lang="en">Italian Digital Transformation Team</dc:creator>
        <rdfs:comment xml:lang="en">This is the ontology of the Italian application profile for Person</rdfs:comment>
        <owl:versionInfo xml:lang="en">Version 0.2 - 08  August 2017 - exclusion of Location part of the ontology since it is included in the related ontology</owl:versionInfo>
        <dc:creator xml:lang="it">Agenzia per l&apos;italia Digitale (AgID)</dc:creator>
        <dc:creator xml:lang="it">Istituto di Scienze e Tecnologie della Cognizione dell&apos;Istituto nazionale delle Ricerche (CNR) - Laboratorio di Tecnologie Semantiche (STlab)</dc:creator>
        <rdfs:comment xml:lang="it">Questa è l&apos;ontologia del profilo applicativo italiano sulle persone.</rdfs:comment>
        <dc:creator xml:lang="it">Team per la Trasformazione Digitale</dc:creator>
        <owl:versionInfo xml:lang="it">Versione 0.2 - 08 Agosto 2017 - separata la parte luoghi dall&apos;ontologia persone</owl:versionInfo>
        <owl:versionIRI rdf:resource="http://dati.gov.it/onto/cpvapit/0.3"/>
        <owl:imports rdf:resource="http://dati.gov.it/onto/l0/"/>
        <rdfs:isDefinedBy rdf:resource="http://dati.gov.it/onto/person/"/>
        <prov:wasDerivedFrom rdf:resource="http://dati.gov.it/onto/person/0.1"/>
        <dct:license rdf:resource="https://creativecommons.org/licenses/by/4.0/"/>
    </owl:Ontology>
    


    <!-- 
    ///////////////////////////////////////////////////////////////////////////////////////
    //
    // Datatypes
    //
    ///////////////////////////////////////////////////////////////////////////////////////
     -->

    


    <!-- http://www.w3.org/2001/XMLSchema#date -->

    <rdfs:Datatype rdf:about="&xsd;date"/>
    


    <!-- 
    ///////////////////////////////////////////////////////////////////////////////////////
    //
    // Object Properties
    //
    ///////////////////////////////////////////////////////////////////////////////////////
     -->

    


    <!-- http://dati.gov.it/onto/cpvapit/hasAddress -->

    <owl:ObjectProperty rdf:about="http://dati.gov.it/onto/cpvapit/hasAddress">
        <rdfs:label xml:lang="en">The address associated with a person.</rdfs:label>
        <rdfs:label xml:lang="en">has address</rdfs:label>
        <rdfs:label xml:lang="it">L&apos;indirizzo associato ad una persona.</rdfs:label>
        <rdfs:label xml:lang="it">ha indirizzo</rdfs:label>
        <rdfs:domain rdf:resource="http://dati.gov.it/onto/cpvapit/Person"/>
        <rdfs:range rdf:resource="&l0;Location"/>
        <rdfs:subPropertyOf rdf:resource="&owl;topObjectProperty"/>
    </owl:ObjectProperty>
    


    <!-- http://dati.gov.it/onto/cpvapit/hasBirthPalce -->

    <owl:ObjectProperty rdf:about="http://dati.gov.it/onto/cpvapit/hasBirthPalce">
        <rdfs:label xml:lang="en">birth place</rdfs:label>
        <rdfs:label xml:lang="it">luogo di nascita</rdfs:label>
        <rdfs:comment xml:lang="en">The relation asserts that a person has a certain place of birth.</rdfs:comment>
        <rdfs:comment xml:lang="it">La relazione che permette di asserire che una persona è nata in un certo luogo.</rdfs:comment>
        <rdfs:domain rdf:resource="http://dati.gov.it/onto/cpvapit/Person"/>
        <rdfs:range rdf:resource="&l0;Location"/>
    </owl:ObjectProperty>
    


    <!-- http://dati.gov.it/onto/cpvapit/hasCitizenship -->

    <owl:ObjectProperty rdf:about="http://dati.gov.it/onto/cpvapit/hasCitizenship">
        <rdfs:label xml:lang="en">citizenship</rdfs:label>
        <rdfs:label xml:lang="it">cittadinanza</rdfs:label>
        <rdfs:comment xml:lang="en">The citizenship of a person (e.g. Italian)</rdfs:comment>
        <rdfs:comment xml:lang="it">La cittadinanza di una persona (ex. cittadinanza italiana).</rdfs:comment>
    </owl:ObjectProperty>
    


    <!-- http://dati.gov.it/onto/cpvapit/hasDeathPlace -->

    <owl:ObjectProperty rdf:about="http://dati.gov.it/onto/cpvapit/hasDeathPlace">
        <rdfs:label xml:lang="en">death place</rdfs:label>
        <rdfs:label xml:lang="it">luogo di morte</rdfs:label>
        <rdfs:comment xml:lang="en">A person&apos;s place of death.</rdfs:comment>
        <rdfs:comment xml:lang="it">Il luogo di morte di una persona.</rdfs:comment>
        <rdfs:domain rdf:resource="http://dati.gov.it/onto/cpvapit/Person"/>
        <rdfs:range rdf:resource="&l0;Location"/>
    </owl:ObjectProperty>
    


    <!-- http://dati.gov.it/onto/cpvapit/hasParentalRelationshipWith -->

    <owl:ObjectProperty rdf:about="http://dati.gov.it/onto/cpvapit/hasParentalRelationshipWith">
        <rdfs:label xml:lang="en">has parental relationship with</rdfs:label>
        <rdfs:label xml:lang="it">ha relazione parentale con</rdfs:label>
        <rdfs:comment xml:lang="en">A parental relationship between two persons.</rdfs:comment>
        <rdfs:comment xml:lang="it">Una relazione di parentela tra due persone.</rdfs:comment>
        <rdfs:subPropertyOf rdf:resource="http://dati.gov.it/onto/cpvapit/hasRelationshipWith"/>
    </owl:ObjectProperty>
    


    <!-- http://dati.gov.it/onto/cpvapit/hasRelationshipWith -->

    <owl:ObjectProperty rdf:about="http://dati.gov.it/onto/cpvapit/hasRelationshipWith">
        <rdfs:label xml:lang="en">has relationship with</rdfs:label>
        <rdfs:label xml:lang="it">ha relazione con</rdfs:label>
        <rdfs:comment xml:lang="en">Any relationship between agents.</rdfs:comment>
        <rdfs:comment xml:lang="it">Qualsiasi relazione tra agenti.</rdfs:comment>
        <rdfs:domain rdf:resource="http://dati.gov.it/onto/cpvapit/Person"/>
        <rdfs:range rdf:resource="http://dati.gov.it/onto/cpvapit/Person"/>
    </owl:ObjectProperty>
    


    <!-- http://dati.gov.it/onto/cpvapit/isBirthPlaceOf -->

    <owl:ObjectProperty rdf:about="http://dati.gov.it/onto/cpvapit/isBirthPlaceOf">
        <rdfs:label xml:lang="en">is birth place of</rdfs:label>
        <rdfs:label xml:lang="it">è luogo di nascita di</rdfs:label>
        <rdfs:comment xml:lang="en">The relation between a place and a person. The relation asserts that a place is the place of birth of the person object of the relation.</rdfs:comment>
        <rdfs:comment xml:lang="it">La relazione tra un luogo ed una persona dove il luogo è il soggetto e la persona l&apos;oggetto della relazione.</rdfs:comment>
        <rdfs:range rdf:resource="http://dati.gov.it/onto/cpvapit/Person"/>
        <owl:inverseOf rdf:resource="http://dati.gov.it/onto/cpvapit/hasBirthPalce"/>
        <rdfs:domain rdf:resource="&l0;Location"/>
    </owl:ObjectProperty>
    


    <!-- http://dati.gov.it/onto/cpvapit/isChildOf -->

    <owl:ObjectProperty rdf:about="http://dati.gov.it/onto/cpvapit/isChildOf">
        <rdfs:label xml:lang="en">child of</rdfs:label>
        <rdfs:label xml:lang="it">figlio di</rdfs:label>
        <rdfs:comment xml:lang="en">The relation child-parent (e.g. John is the son of Peter).</rdfs:comment>
        <rdfs:comment xml:lang="it">La relazione figlio-padre (ex. Mario è figlio di Carlo).</rdfs:comment>
        <rdfs:domain rdf:resource="http://dati.gov.it/onto/cpvapit/Person"/>
        <rdfs:range rdf:resource="http://dati.gov.it/onto/cpvapit/Person"/>
        <rdfs:subPropertyOf rdf:resource="http://dati.gov.it/onto/cpvapit/hasParentalRelationshipWith"/>
    </owl:ObjectProperty>
    


    <!-- http://dati.gov.it/onto/cpvapit/isDeathPlaceOf -->

    <owl:ObjectProperty rdf:about="http://dati.gov.it/onto/cpvapit/isDeathPlaceOf">
        <rdfs:label xml:lang="en">death place of</rdfs:label>
        <rdfs:label xml:lang="it">luogo di morte di</rdfs:label>
        <rdfs:comment xml:lang="en">The property to associate a death place (i.e. a location) with a person.</rdfs:comment>
        <rdfs:comment xml:lang="it">La proprietà per associare un luogo (i.e. una località) ad una persona a persona per rappresentare il luogo di morte di quest&apos;ultima.</rdfs:comment>
        <rdfs:range rdf:resource="http://dati.gov.it/onto/cpvapit/Person"/>
        <owl:inverseOf rdf:resource="http://dati.gov.it/onto/cpvapit/hasDeathPlace"/>
        <rdfs:domain rdf:resource="&l0;Location"/>
    </owl:ObjectProperty>
    


    <!-- http://dati.gov.it/onto/cpvapit/isNephewOf -->

    <owl:ObjectProperty rdf:about="http://dati.gov.it/onto/cpvapit/isNephewOf">
        <rdfs:label xml:lang="en">is nephew of</rdfs:label>
        <rdfs:label xml:lang="it">è nipote di</rdfs:label>
        <rdfs:comment xml:lang="en">The nephew relation between a newphew and an uncle.</rdfs:comment>
        <rdfs:comment xml:lang="it">La relazione di parentela tra un nipote ed uno zio.</rdfs:comment>
        <rdfs:subPropertyOf rdf:resource="http://dati.gov.it/onto/cpvapit/hasParentalRelationshipWith"/>
        <owl:inverseOf rdf:resource="http://dati.gov.it/onto/cpvapit/isUncleOf"/>
    </owl:ObjectProperty>
    


    <!-- http://dati.gov.it/onto/cpvapit/isParentOf -->

    <owl:ObjectProperty rdf:about="http://dati.gov.it/onto/cpvapit/isParentOf">
        <rdfs:label xml:lang="en">The parent-child relationship.</rdfs:label>
        <rdfs:label xml:lang="en">is parent of</rdfs:label>
        <rdfs:label xml:lang="it">La relazione padre-figlio.</rdfs:label>
        <rdfs:label xml:lang="it">è genitore di</rdfs:label>
        <rdfs:domain rdf:resource="http://dati.gov.it/onto/cpvapit/Person"/>
        <rdfs:range rdf:resource="http://dati.gov.it/onto/cpvapit/Person"/>
        <rdfs:subPropertyOf rdf:resource="http://dati.gov.it/onto/cpvapit/hasParentalRelationshipWith"/>
        <owl:inverseOf rdf:resource="http://dati.gov.it/onto/cpvapit/isChildOf"/>
    </owl:ObjectProperty>
    


    <!-- http://dati.gov.it/onto/cpvapit/isUncleOf -->

    <owl:ObjectProperty rdf:about="http://dati.gov.it/onto/cpvapit/isUncleOf">
        <rdfs:label xml:lang="en">The uncleship relation.</rdfs:label>
        <rdfs:label xml:lang="en">is uncle of</rdfs:label>
        <rdfs:label xml:lang="it">è zio di</rdfs:label>
        <rdfs:comment xml:lang="it">La relazione di parentela tra zio e nipote.</rdfs:comment>
        <rdfs:range rdf:resource="http://dati.gov.it/onto/cpvapit/Person"/>
        <rdfs:domain rdf:resource="http://dati.gov.it/onto/cpvapit/Person"/>
        <rdfs:subPropertyOf rdf:resource="http://dati.gov.it/onto/cpvapit/hasParentalRelationshipWith"/>
    </owl:ObjectProperty>
    


    <!-- http://dati.gov.it/onto/cpvapit/knows -->

    <owl:ObjectProperty rdf:about="http://dati.gov.it/onto/cpvapit/knows">
        <rdf:type rdf:resource="&owl;SymmetricProperty"/>
        <rdfs:label xml:lang="en">knows</rdfs:label>
        <rdfs:label xml:lang="it">conosce</rdfs:label>
        <rdfs:comment xml:lang="en">The relationship of knowledge between two people. E.g. &apos;John White&apos; knows &apos;Bob Black&apos;.</rdfs:comment>
        <rdfs:comment xml:lang="it">La relazione di conoscenza che intercorre tra due persone. Ex. &apos;Mario Rossi&apos; conosce &apos;Paolo Neri&apos;.</rdfs:comment>
        <rdfs:range rdf:resource="http://dati.gov.it/onto/cpvapit/Person"/>
        <rdfs:domain rdf:resource="http://dati.gov.it/onto/cpvapit/Person"/>
        <rdfs:subPropertyOf rdf:resource="http://dati.gov.it/onto/cpvapit/hasRelationshipWith"/>
    </owl:ObjectProperty>
    


    <!-- 
    ///////////////////////////////////////////////////////////////////////////////////////
    //
    // Data properties
    //
    ///////////////////////////////////////////////////////////////////////////////////////
     -->

    


    <!-- http://dati.gov.it/onto/cpvapit/altName -->

    <owl:DatatypeProperty rdf:about="http://dati.gov.it/onto/cpvapit/altName">
        <rdfs:range rdf:resource="&xsd;string"/>
        <rdfs:domain rdf:resource="&owl;Thing"/>
    </owl:DatatypeProperty>
    


    <!-- http://dati.gov.it/onto/cpvapit/birthDate -->

    <owl:DatatypeProperty rdf:about="http://dati.gov.it/onto/cpvapit/birthDate">
        <rdfs:domain rdf:resource="http://dati.gov.it/onto/cpvapit/Person"/>
        <rdfs:range rdf:resource="&xsd;date"/>
    </owl:DatatypeProperty>
    


    <!-- http://dati.gov.it/onto/cpvapit/familyName -->

    <owl:DatatypeProperty rdf:about="http://dati.gov.it/onto/cpvapit/familyName">
        <rdfs:label xml:lang="en">family name</rdfs:label>
        <rdfs:label xml:lang="it">cognome</rdfs:label>
        <rdfs:comment xml:lang="en">The family name of a person. E.g. &apos;Rossi&apos; is the family name of the person &apos;Mario Rossi&apos;.</rdfs:comment>
        <rdfs:comment xml:lang="it">Il cognome di una persona. Ex. &apos;Rossi&apos; è il cognome della persona &apos;Mario Rossi&apos;</rdfs:comment>
        <rdfs:domain rdf:resource="http://dati.gov.it/onto/cpvapit/Person"/>
        <rdfs:range rdf:resource="&xsd;string"/>
    </owl:DatatypeProperty>
    


    <!-- http://dati.gov.it/onto/cpvapit/givenName -->

    <owl:DatatypeProperty rdf:about="http://dati.gov.it/onto/cpvapit/givenName">
        <rdfs:label xml:lang="en">given name</rdfs:label>
        <rdfs:label xml:lang="it">nome</rdfs:label>
        <rdfs:comment xml:lang="en">The given name of a person. E.g. &apos;Mario&apos; is the given name of the person &apos;Mario Rossi&apos;.</rdfs:comment>
        <rdfs:comment xml:lang="it">Il nome di una persona. Ex. &apos;Mario&apos; è il nome della persona &apos;Mario Rossi&apos;.</rdfs:comment>
        <rdfs:domain rdf:resource="http://dati.gov.it/onto/cpvapit/Person"/>
        <rdfs:range rdf:resource="&xsd;string"/>
    </owl:DatatypeProperty>
    


    <!-- http://dati.gov.it/onto/cpvapit/identifier -->

    <owl:DatatypeProperty rdf:about="http://dati.gov.it/onto/cpvapit/identifier">
        <rdfs:range rdf:resource="&rdfs;Literal"/>
        <rdfs:domain rdf:resource="&owl;Thing"/>
    </owl:DatatypeProperty>
    


    <!-- http://dati.gov.it/onto/cpvapit/name -->

    <owl:DatatypeProperty rdf:about="http://dati.gov.it/onto/cpvapit/name">
        <rdfs:label xml:lang="en">name</rdfs:label>
        <rdfs:label xml:lang="it">nome</rdfs:label>
        <rdfs:comment xml:lang="en">The name used for referencing any individual of the class Agent. E.g. &apos;Mario Rossi&apos; is the name of the person &apos;Mario Rossi&apos; or &apos;CNR&apos; is one of the possible alternatives used for referencing the National Italian Council for Research.</rdfs:comment>
        <rdfs:comment xml:lang="it">Il nome con cui ci si referisce ad un individiduo della classe Agent. Ex. &apos;Mario Rossi&apos; è il nome della persona &apos;Mario Rossi&apos; oppure &apos;CNR&apos; è uno dei possibili nomi con cui ci si riferisce al Consiglio Nazionale delle Ricerche.</rdfs:comment>
        <rdfs:range rdf:resource="&xsd;string"/>
    </owl:DatatypeProperty>
    


    <!-- 
    ///////////////////////////////////////////////////////////////////////////////////////
    //
    // Classes
    //
    ///////////////////////////////////////////////////////////////////////////////////////
     -->

    


    <!-- http://dati.gov.it/onto/cpvapit/Person -->

    <owl:Class rdf:about="http://dati.gov.it/onto/cpvapit/Person">
        <rdfs:label xml:lang="en">Person</rdfs:label>
        <rdfs:label xml:lang="it">Persona</rdfs:label>
        <rdfs:subClassOf rdf:resource="&l0;Agent"/>
        <rdfs:comment xml:lang="en">A natural person</rdfs:comment>
        <rdfs:comment xml:lang="it">Una persona naturale</rdfs:comment>
    </owl:Class>
</rdf:RDF>



<!-- Generated by the OWL API (version 3.5.1) http://owlapi.sourceforge.net -->

