<?xml version="1.0" encoding="UTF-8"?>
<rdf:RDF
   xmlns:dc="http://purl.org/dc/elements/1.1/"
   xmlns:dct="http://purl.org/dc/terms/"
   xmlns:owl="http://www.w3.org/2002/07/owl#"
   xmlns:prov="http://www.w3.org/ns/prov#"
   xmlns:rdf="http://www.w3.org/1999/02/22-rdf-syntax-ns#"
   xmlns:rdfs="http://www.w3.org/2000/01/rdf-schema#"
>
  <rdf:Description rdf:about="http://dati.gov.it/onto/l0/Agent">
    <rdfs:comment xml:lang="it">Un agente, sia fisico (ex. una persona, un robot, una quercia), o sociale (ex. una società, un'istituzione, una comunità).</rdfs:comment>
    <rdf:type rdf:resource="http://www.w3.org/2002/07/owl#Class"/>
    <rdfs:label xml:lang="it">Agente</rdfs:label>
    <rdfs:subClassOf rdf:resource="http://dati.gov.it/onto/l0/Entity"/>
    <rdfs:comment xml:lang="en">Any agentive Object , either physical (e.g. a person, a robot, an oak), or social (e.g. a corporation, an institution, a community).</rdfs:comment>
    <rdfs:label xml:lang="en">Agent</rdfs:label>
  </rdf:Description>
  <rdf:Description rdf:about="http://dati.gov.it/onto/l0/System">
    <rdfs:label xml:lang="it">Sistema</rdfs:label>
    <rdfs:comment xml:lang="en">This class represents a system. Example of systems are politacal or economical systems.</rdfs:comment>
    <rdf:type rdf:resource="http://www.w3.org/2002/07/owl#Class"/>
    <rdfs:comment xml:lang="it">Questa classe rappresenta un sistema. Esempi di sistema sono un sistema politico o economico.</rdfs:comment>
    <rdfs:label xml:lang="en">System</rdfs:label>
  </rdf:Description>
  <rdf:Description rdf:about="http://dati.gov.it/onto/l0/Topic">
    <rdf:type rdf:resource="http://www.w3.org/2002/07/owl#Class"/>
    <rdfs:label xml:lang="en">Topic</rdfs:label>
    <rdfs:comment xml:lang="en">The concept of topic.</rdfs:comment>
    <rdfs:label xml:lang="it">Tema</rdfs:label>
    <rdfs:comment xml:lang="it">Il concetto di tema o argomento.</rdfs:comment>
  </rdf:Description>
  <rdf:Description rdf:about="http://dati.gov.it/onto/l0/Event">
    <rdfs:label xml:lang="it">Evento</rdfs:label>
    <rdf:type rdf:resource="http://www.w3.org/2002/07/owl#Class"/>
    <rdfs:comment xml:lang="en">Representation of the concept of event.</rdfs:comment>
    <rdfs:label xml:lang="en">Event</rdfs:label>
    <rdfs:comment xml:lang="it">Rappresentazione del concetto di evento.</rdfs:comment>
  </rdf:Description>
  <rdf:Description rdf:about="http://dati.gov.it/onto/l0/">
    <rdfs:comment xml:lang="en">This ontology provides the foundational level of the ontological stack of dati.gov.it. The name L0 stands for Level-0 ontology as it provides the basic conceptual foundations to the whole stack. This ontology is partially inspired by DOLCE 0 (http://www.ontologydesignpatterns.org/ont/d0.owl)</rdfs:comment>
    <rdf:type rdf:resource="http://www.w3.org/2002/07/owl#Ontology"/>
    <owl:verionInfo>0.2 - aggiunto il seguente assioma: Location sottoclasse di Entity e aggiunto un collegamento con DOLCE 0.</owl:verionInfo>
    <dc:creator xml:lang="en">Institute of Cognitive Sciences and Technologies of the Italian Research Council (CNR) - Semantic Technology Laboratory (STLab)</dc:creator>
    <rdfs:comment xml:lang="it">Questa ontologia fornisce il livello fondazionale allo stack ontologico di dati.gov.it. Il nome L0 sta per Level-0 ontology poiché essa fornisce le fondamenta concettuali elementari all'intero stack. Questa ontologia è parzialmente ispirata da DOLCE zero (http://www.ontologydesignpatterns.org/ont/d0.owl)</rdfs:comment>
    <prov:wasInfluencedBy rdf:resource="http://www.ontologydesignpatterns.org/ont/d0.owl"/>
    <dc:creator xml:lang="en">Agency for Digital Italy - AgID</dc:creator>
    <owl:versionInfo xml:lang="en">0.2 - added the following axiom: Location subclass of Entity; added soft link with DOLCE 0</owl:versionInfo>
    <rdfs:label xml:lang="en">Level-0 ontology</rdfs:label>
    <rdfs:label xml:lang="it">Ontologia Level-0</rdfs:label>
    <dct:modified>2017-10-18</dct:modified>
    <dc:creator xml:lang="en">Italian Digital Transformation Team</dc:creator>
    <dct:issued>2017-09-29</dct:issued>
  </rdf:Description>
  <rdf:Description rdf:about="http://dati.gov.it/onto/l0/Activity">
    <rdfs:comment xml:lang="it">La classe che rappresenta un'attività.</rdfs:comment>
    <rdf:type rdf:resource="http://www.w3.org/2002/07/owl#Class"/>
    <rdfs:comment xml:lang="en">The class whose that models an activity.</rdfs:comment>
    <rdfs:label xml:lang="it">Attività</rdfs:label>
    <rdfs:label xml:lang="en">Activity</rdfs:label>
  </rdf:Description>
  <rdf:Description rdf:about="http://dati.gov.it/onto/l0/Location">
    <rdfs:subClassOf rdf:resource="http://dati.gov.it/onto/l0/Entity"/>
    <rdf:type rdf:resource="http://www.w3.org/2002/07/owl#Class"/>
    <rdfs:label xml:lang="en">Location</rdfs:label>
    <rdfs:comment xml:lang="it">Classe che rappresenta il concetto di luogo. Le istanze di questa classe sono, pertanto, luoghi.</rdfs:comment>
    <rdfs:label xml:lang="it">Luogo</rdfs:label>
    <rdfs:comment xml:lang="en">The class that reprepresents a location. Individuals of this class are locations (e.g. geographical places, spacial objects, etc.).</rdfs:comment>
  </rdf:Description>
  <rdf:Description rdf:about="http://dati.gov.it/onto/l0/Collection">
    <rdfs:label xml:lang="it">Collezione</rdfs:label>
    <rdfs:label xml:lang="en">Collection</rdfs:label>
    <rdf:type rdf:resource="http://www.w3.org/2002/07/owl#Class"/>
    <rdfs:comment xml:lang="it">La classe che rappresenta una collezione di qualsiasi cosa.</rdfs:comment>
    <rdfs:comment xml:lang="en">The class that represents a collection of things.</rdfs:comment>
  </rdf:Description>
  <rdf:Description rdf:about="http://www.w3.org/ns/prov#wasInfluencedBy">
    <rdf:type rdf:resource="http://www.w3.org/2002/07/owl#AnnotationProperty"/>
  </rdf:Description>
  <rdf:Description rdf:about="http://dati.gov.it/onto/l0/Characteristic">
    <rdfs:comment xml:lang="it">Questa classe rappresenta una caratteristica.</rdfs:comment>
    <rdfs:label xml:lang="en">Characteristic</rdfs:label>
    <rdf:type rdf:resource="http://www.w3.org/2002/07/owl#Class"/>
    <rdfs:comment xml:lang="en">This class represent a characteristic.</rdfs:comment>
    <rdfs:label xml:lang="it">Caratteristica</rdfs:label>
  </rdf:Description>
  <rdf:Description rdf:about="http://dati.gov.it/onto/l0/Entity">
    <rdfs:comment xml:lang="it">Qualsiasi cosa reale, possibile o immaginaria.</rdfs:comment>
    <rdfs:comment xml:lang="en">Anything: real, possible, or imaginary, which some modeller wants to talk about for some purpose.</rdfs:comment>
    <rdf:type rdf:resource="http://www.w3.org/2002/07/owl#Class"/>
    <rdfs:label xml:lang="en">Entity</rdfs:label>
    <rdfs:label xml:lang="it">Entità</rdfs:label>
  </rdf:Description>
  <rdf:Description rdf:about="http://dati.gov.it/onto/l0/Object">
    <rdfs:label xml:lang="it">Oggetto</rdfs:label>
    <rdf:type rdf:resource="http://www.w3.org/2002/07/owl#Class"/>
    <rdfs:comment xml:lang="en">An object.</rdfs:comment>
    <rdfs:label xml:lang="en">Object</rdfs:label>
    <rdfs:subClassOf rdf:resource="http://dati.gov.it/onto/l0/Entity"/>
    <rdfs:comment xml:lang="it">Un oggetto.</rdfs:comment>
  </rdf:Description>
</rdf:RDF>
