<?xml version="1.0"?>
<rdf:RDF xmlns="https://w3id.org/italia/onto/Transparency/"
     xml:base="https://w3id.org/italia/onto/Transparency/"
     xmlns:admsapit="https://w3id.org/italia/onto/ADMS/"
     xmlns:l0="https://w3id.org/italia/onto/l0/"
     xmlns:adms="http://www.w3.org/ns/adms#"
     xmlns:owl="http://www.w3.org/2002/07/owl#"
     xmlns:clvapit="https://w3id.org/italia/onto/CLV/"
     xmlns:tiapit="https://w3id.org/italia/onto/TI/"
     xmlns:xsd="http://www.w3.org/2001/XMLSchema#"
     xmlns:skos="http://www.w3.org/2004/02/skos/core#"
     xmlns:rdfs="http://www.w3.org/2000/01/rdf-schema#"
     xmlns:vcard="http://www.w3.org/2006/vcard/ns#"
     xmlns:xkos="http://rdf-vocabulary.ddialliance.org/xkos#"
     xmlns:cpsvapit="https://w3id.org/italia/onto/CPSV/"
     xmlns:dct="http://purl.org/dc/terms/"
     xmlns:rdf="http://www.w3.org/1999/02/22-rdf-syntax-ns#"
     xmlns:xml="http://www.w3.org/XML/1998/namespace"
     xmlns:dcatapit="http://dati.gov.it/onto/dcatapit#"
     xmlns:covapit="https://w3id.org/italia/onto/COV/"
     xmlns:dcat="http://www.w3.org/ns/dcat#"
     xmlns:foaf="http://xmlns.com/foaf/0.1/"
     xmlns:smapit="https://w3id.org/italia/onto/SM/"
     xmlns:dc="http://purl.org/dc/elements/1.1/">
    <owl:Ontology rdf:about="https://w3id.org/italia/onto/Transparency/">
        <owl:versionIRI rdf:resource="https://w3id.org/italia/onto/Transparency/0.1"/>
        <dcat:keyword xml:lang="en">transparency for public administration</dcat:keyword>
        <dct:creator rdf:resource="http://spcdata.digitpa.gov.it/Amministrazione/agid"/>
        <admsapit:target xml:lang="it">Cittadini</admsapit:target>
        <dct:issued rdf:datatype="http://www.w3.org/2001/XMLSchema#date">2019-03-04</dct:issued>
        <admsapit:hasTask rdf:resource="https://w3id.org/italia/onto/ADMS/AnnotationTask"/>
        <admsapit:hasTask rdf:resource="https://w3id.org/italia/onto/ADMS/QueryFormulationTask"/>
        <dcat:keyword xml:lang="it">trasparenza</dcat:keyword>
        <rdfs:comment xml:lang="it">Questo è il profilo applicativo italiano dell&apos;ontologia sull&apos;amministrazione trasparente. L&apos;ontologia di OntoPiA implementa le disposizioni in merito all&apos;obbligo di pubblicazione di contenuti informativi nella sezione &apos;Amministrazione Trasparente&apos; dei siti istituzionali delle publiche amministrazioni.</rdfs:comment>
        <dcat:keyword xml:lang="en">transparency</dcat:keyword>
        <admsapit:prefix>trapit</admsapit:prefix>
        <rdfs:label xml:lang="en">Transparent Administration Ontology - Italian application profile</rdfs:label>
        <admsapit:hasTask rdf:resource="https://w3id.org/italia/onto/ADMS/SearchTask"/>
        <dcat:keyword xml:lang="it">trasparenza PA</dcat:keyword>
        <dcat:keyword xml:lang="it">trasparenza pa</dcat:keyword>
        <rdfs:comment xml:lang="en">This ontology version is a draft waiting for the ANAC validation.</rdfs:comment>
        <admsapit:hasOntologyLanguage rdf:resource="https://w3id.org/italia/onto/ADMS/OWL"/>
        <admsapit:status>draft</admsapit:status>
        <rdfs:comment>Questa versione dell&apos;ontologia è in attesa di essere visionata da ANAC.@it</rdfs:comment>
        <admsapit:officialURI rdf:datatype="http://www.w3.org/2001/XMLSchema#anyURI">https://w3id.org/italia/onto/Transparency</admsapit:officialURI>
        <dct:modified rdf:datatype="http://www.w3.org/2001/XMLSchema#date">2019-03-04</dct:modified>
        <admsapit:acronym>Transparency-AP_IT</admsapit:acronym>
        <dct:description xml:lang="en">This ontology version is a draft waiting for the ANAC validation.</dct:description>
        <owl:versionInfo xml:lang="it">La presente versione dell&apos;ontologia è un draft in attesa di revisone da parte di ANAC.</owl:versionInfo>
        <dct:language rdf:resource="http://publications.europa.eu/resource/authority/language/ENG"/>
        <admsapit:hasFormalityLevel rdf:resource="https://w3id.org/italia/onto/ADMS/Formal"/>
        <dct:rightsHolder rdf:resource="http://spcdata.digitpa.gov.it/Amministrazione/agid"/>
        <admsapit:target xml:lang="it">Pubbliche amministrazioni</admsapit:target>
        <dct:description rdf:resource="https://w3id.org/italia/onto/Transparency/./latest/img/Transparency-AP_IT.png"/>
        <dct:publisher rdf:resource="http://spcdata.digitpa.gov.it/Amministrazione/agid"/>
        <admsapit:hasSemanticAssetDistribution rdf:resource="https://w3id.org/italia/data/distribution/TRAPIT-JSON-LD"/>
        <dct:description xml:lang="it">Questo è il profilo applicativo italiano dell&apos;ontologia sull&apos;amministrazione trasparente. L&apos;ontologia di OntoPiA implementa le disposizioni in merito all&apos;obbligo di pubblicazione di contenuti informativi nella sezione &apos;Amministrazione Trasparente&apos; dei siti istituzioonali delle publiche amministrazioni.</dct:description>
        <dcat:contactPoint rdf:resource="http://dati.gov.it/data/resource/ContactPoint/voc_AgID"/>
        <dct:creator rdf:resource="https://w3id.org/italia/data/organization/private-organization/05481840964"/>
        <admsapit:semanticAssetInUse rdf:resource="https://w3id.org/italia/data/project/DAF"/>
        <admsapit:semanticAssetInUse rdf:resource="https://w3id.org/italia/data/project/OntoPiA"/>
        <dct:accrualPeriodicity rdf:resource="http://publications.europa.eu/resource/authority/frequency/IRREG"/>
        <admsapit:hasSemanticAssetDistribution rdf:resource="https://w3id.org/italia/data/distribution/TRAPIT-RDF-XML"/>
        <dct:title xml:lang="it">Ontologia dell&apos;Amministrazione Trasparente - profilo applicativo italiano</dct:title>
        <rdfs:isDefinedBy rdf:resource="https://w3id.org/italia/onto/Transparency"/>
        <rdfs:comment xml:lang="en">This is the Italian application profile of the ontology on the transparent administration. This ontology of OntoPiA implements the dispositions about the publication obligation of informative contents on the section &apos;Transparent Administration&apos; of the official website of the public administrations.</rdfs:comment>
        <dct:description>Questa versione dell&apos;ontologia è in attesa di essere visionata da ANAC.@it</dct:description>
        <dcat:theme rdf:resource="http://publications.europa.eu/resource/authority/data-theme/GOVE"/>
        <rdfs:label xml:lang="it">Ontologia dell&apos;Amministrazione Trasparente - profilo applicativo italiano</rdfs:label>
        <dct:description xml:lang="en">This is the Italian application profile of the ontology on the transparent administration. This ontology of OntoPiA implements the dispositions about the publication obligation of informative contents on the section &apos;Transparent Administration&apos; of the official website of the public administrations.</dct:description>
        <admsapit:last rdf:resource="https://w3id.org/italia/onto/Transparency/0.1"/>
        <dct:language rdf:resource="http://publications.europa.eu/resource/authority/language/ITA"/>
        <admsapit:hasSemanticAssetDistribution rdf:resource="https://w3id.org/italia/data/distribution/TRAPIT-RDF-TURTLE"/>
        <admsapit:type rdf:resource="https://w3id.org/italia/onto/ADMS/DomainOntology"/>
        <dcat:theme rdf:resource="http://publications.europa.eu/resource/authority/data-theme/TECH"/>
        <dcat:keyword xml:lang="it">trasparenza pubblica amministrazione</dcat:keyword>
    </owl:Ontology>
    


    <!-- 
    ///////////////////////////////////////////////////////////////////////////////////////
    //
    // Annotation properties
    //
    ///////////////////////////////////////////////////////////////////////////////////////
     -->

    


    <!-- http://purl.org/dc/terms/description -->

    <owl:AnnotationProperty rdf:about="http://purl.org/dc/terms/description"/>
    


    <!-- http://purl.org/dc/terms/format -->

    <owl:AnnotationProperty rdf:about="http://purl.org/dc/terms/format"/>
    


    <!-- http://purl.org/dc/terms/identifier -->

    <owl:AnnotationProperty rdf:about="http://purl.org/dc/terms/identifier"/>
    


    <!-- http://purl.org/dc/terms/license -->

    <owl:AnnotationProperty rdf:about="http://purl.org/dc/terms/license"/>
    


    <!-- http://purl.org/dc/terms/title -->

    <owl:AnnotationProperty rdf:about="http://purl.org/dc/terms/title"/>
    


    <!-- http://www.w3.org/ns/dcat#accessURL -->

    <owl:AnnotationProperty rdf:about="http://www.w3.org/ns/dcat#accessURL"/>
    


    <!-- http://www.w3.org/ns/dcat#downloadURL -->

    <owl:AnnotationProperty rdf:about="http://www.w3.org/ns/dcat#downloadURL"/>
    


    <!-- http://xmlns.com/foaf/0.1/name -->

    <owl:AnnotationProperty rdf:about="http://xmlns.com/foaf/0.1/name"/>
    


    <!-- https://w3id.org/italia/onto/l0/controlledVocabulary -->

    <owl:AnnotationProperty rdf:about="https://w3id.org/italia/onto/l0/controlledVocabulary"/>
    


    <!-- 
    ///////////////////////////////////////////////////////////////////////////////////////
    //
    // Datatypes
    //
    ///////////////////////////////////////////////////////////////////////////////////////
     -->

    


    <!-- http://www.w3.org/2001/XMLSchema#date -->

    <rdfs:Datatype rdf:about="http://www.w3.org/2001/XMLSchema#date"/>
    


    <!-- 
    ///////////////////////////////////////////////////////////////////////////////////////
    //
    // Object Properties
    //
    ///////////////////////////////////////////////////////////////////////////////////////
     -->

    


    <!-- https://w3id.org/italia/onto/Transparency/accrualPeriodicity -->

    <owl:ObjectProperty rdf:about="https://w3id.org/italia/onto/Transparency/accrualPeriodicity">
        <rdfs:domain rdf:resource="https://w3id.org/italia/onto/Transparency/ObligationContent"/>
        <rdfs:range rdf:resource="https://w3id.org/italia/onto/Transparency/Frequency"/>
        <rdfs:comment xml:lang="it">Questa proprietà lega un obbligo di trasparenza alla frequenza con cui va aggiornato il contenuto. vedi dcatapit.</rdfs:comment>
        <rdfs:comment xml:lang="en">This property links a transparency obligation to the update frequency of the content.</rdfs:comment>
        <rdfs:isDefinedBy rdf:resource="https://w3id.org/italia/onto/Transparency/"/>
        <rdfs:label xml:lang="en">accrual periodicity</rdfs:label>
        <rdfs:label xml:lang="it">frequenza di aggiornamento</rdfs:label>
    </owl:ObjectProperty>
    


    <!-- https://w3id.org/italia/onto/Transparency/affects -->

    <owl:ObjectProperty rdf:about="https://w3id.org/italia/onto/Transparency/affects">
        <owl:inverseOf rdf:resource="https://w3id.org/italia/onto/Transparency/isObjectOfObligation"/>
        <rdfs:domain rdf:resource="https://w3id.org/italia/onto/Transparency/TransparencySubject"/>
        <rdfs:range rdf:resource="https://w3id.org/italia/onto/Transparency/TransparencyObligation"/>
        <rdfs:comment xml:lang="it">Questa proprietà lega obbligo di trasparenza al soggetto che lo riguarda.</rdfs:comment>
        <rdfs:comment xml:lang="en">This property links a transparency obligation to the affected subjects.</rdfs:comment>
        <rdfs:isDefinedBy rdf:resource="https://w3id.org/italia/onto/Transparency/"/>
        <rdfs:label xml:lang="en">is obligation for</rdfs:label>
        <rdfs:label xml:lang="it">è obbligo per</rdfs:label>
    </owl:ObjectProperty>
    


    <!-- https://w3id.org/italia/onto/Transparency/comply -->

    <owl:ObjectProperty rdf:about="https://w3id.org/italia/onto/Transparency/comply">
        <rdfs:domain rdf:resource="https://w3id.org/italia/onto/Transparency/Content"/>
        <rdfs:range rdf:resource="https://w3id.org/italia/onto/Transparency/ObligationContent"/>
        <rdfs:comment xml:lang="it">Questa proprietà lega un contenuto informativo al contenuto del relativo obbligo di trasparenza.</rdfs:comment>
        <rdfs:comment xml:lang="en">This property links a informative content to the related transparency obligation content.</rdfs:comment>
        <rdfs:isDefinedBy rdf:resource="https://w3id.org/italia/onto/Transparency/"/>
        <rdfs:label xml:lang="en">comply</rdfs:label>
        <rdfs:label xml:lang="it">ottempera</rdfs:label>
    </owl:ObjectProperty>
    


    <!-- https://w3id.org/italia/onto/Transparency/hasContent -->

    <owl:ObjectProperty rdf:about="https://w3id.org/italia/onto/Transparency/hasContent">
        <owl:inverseOf rdf:resource="https://w3id.org/italia/onto/Transparency/hasSubject"/>
        <rdfs:domain rdf:resource="https://w3id.org/italia/onto/Transparency/TransparencySubject"/>
        <rdfs:range rdf:resource="https://w3id.org/italia/onto/Transparency/Content"/>
        <rdfs:comment xml:lang="it">Questa proprietà lega un soggetto (i.e. argomento o soggetto fisico)ai contenuto da pubblicare relativi.</rdfs:comment>
        <rdfs:comment xml:lang="en">This property links an informative content to the related subject.</rdfs:comment>
        <rdfs:isDefinedBy rdf:resource="https://w3id.org/italia/onto/Transparency/"/>
        <rdfs:label xml:lang="it">ha contenuto informativo</rdfs:label>
        <rdfs:label xml:lang="en">has informative content</rdfs:label>
    </owl:ObjectProperty>
    


    <!-- https://w3id.org/italia/onto/Transparency/hasObligationContent -->

    <owl:ObjectProperty rdf:about="https://w3id.org/italia/onto/Transparency/hasObligationContent">
        <owl:inverseOf rdf:resource="https://w3id.org/italia/onto/Transparency/isObligationContentOf"/>
        <rdfs:domain rdf:resource="https://w3id.org/italia/onto/Transparency/TransparencyObligation"/>
        <rdfs:range rdf:resource="https://w3id.org/italia/onto/Transparency/ObligationContent"/>
        <rdfs:comment xml:lang="it">Questa proprietà lega un obbligo di trasparenza ai suoi contenuti.</rdfs:comment>
        <rdfs:comment xml:lang="en">This property links a transparency obligation to its contents.</rdfs:comment>
        <rdfs:isDefinedBy rdf:resource="https://w3id.org/italia/onto/Transparency/"/>
        <rdfs:label xml:lang="it">ha contenuto obbligo</rdfs:label>
        <rdfs:label xml:lang="en">has content of obligation</rdfs:label>
    </owl:ObjectProperty>
    


    <!-- https://w3id.org/italia/onto/Transparency/hasSubject -->

    <owl:ObjectProperty rdf:about="https://w3id.org/italia/onto/Transparency/hasSubject">
        <rdfs:domain rdf:resource="https://w3id.org/italia/onto/Transparency/Content"/>
        <rdfs:range rdf:resource="https://w3id.org/italia/onto/Transparency/TransparencySubject"/>
        <rdfs:comment xml:lang="it">Questa proprietà lega un contenuto informativo all&apos;argomento a cui si riferisce.</rdfs:comment>
        <rdfs:comment xml:lang="en">This property links an informative content to the related subject.</rdfs:comment>
        <rdfs:isDefinedBy rdf:resource="https://w3id.org/italia/onto/Transparency/"/>
        <rdfs:label xml:lang="it">ha argomento</rdfs:label>
        <rdfs:label xml:lang="en">has subject</rdfs:label>
    </owl:ObjectProperty>
    


    <!-- https://w3id.org/italia/onto/Transparency/hasTransparencySubSection -->

    <owl:ObjectProperty rdf:about="https://w3id.org/italia/onto/Transparency/hasTransparencySubSection">
        <rdfs:domain rdf:resource="https://w3id.org/italia/onto/Transparency/TransparencyObligation"/>
        <rdfs:range rdf:resource="https://w3id.org/italia/onto/Transparency/TransparencyTitulus"/>
        <rdfs:comment xml:lang="it">Questa proprietà lega un obbligo di trasparenza alla sotto-sezione di &apos;Amministrazione Trasparente&apos; in cui devono essere pubblicati i suoi contenuti. Le sotto-sezioni sono controllate della tassonomia https://w3id.org/italia/controlled-vocabulary/classifications-for-transparency/transparency-titulus</rdfs:comment>
        <rdfs:comment xml:lang="en">This property links a transparency obligation to the sub-section of the &apos;Transparent Administration&apos; section where the contents must be published. The values are controlled by the taxonomy  https://w3id.org/italia/controlled-vocabulary/classifications-for-transparency/transparency-titulus </rdfs:comment>
        <rdfs:isDefinedBy rdf:resource="https://w3id.org/italia/onto/Transparency/"/>
        <rdfs:label xml:lang="it">ha sotto-sezione obbligo</rdfs:label>
        <rdfs:label xml:lang="en">has transparency sub section</rdfs:label>
    </owl:ObjectProperty>
    


    <!-- https://w3id.org/italia/onto/Transparency/isAppliedTo -->

    <owl:ObjectProperty rdf:about="https://w3id.org/italia/onto/Transparency/isAppliedTo">
        <rdfs:domain rdf:resource="https://w3id.org/italia/onto/Transparency/TransparencyObligation"/>
        <rdfs:range rdf:resource="https://w3id.org/italia/onto/COV/PublicOrganization"/>
        <rdfs:comment xml:lang="it">Questa proprietà lega un obbligo di trasparenza alla pubblica amministrazione a cui si applica.</rdfs:comment>
        <rdfs:comment xml:lang="en">This property links a transparency obligation to a public administration to whom is applied.</rdfs:comment>
        <rdfs:isDefinedBy rdf:resource="https://w3id.org/italia/onto/Transparency/"/>
        <rdfs:label xml:lang="en">is applied to</rdfs:label>
        <rdfs:label xml:lang="it">si applica a</rdfs:label>
    </owl:ObjectProperty>
    


    <!-- https://w3id.org/italia/onto/Transparency/isObjectOfObligation -->

    <owl:ObjectProperty rdf:about="https://w3id.org/italia/onto/Transparency/isObjectOfObligation">
        <rdfs:domain rdf:resource="https://w3id.org/italia/onto/Transparency/TransparencySubject"/>
        <rdfs:range rdf:resource="https://w3id.org/italia/onto/Transparency/TransparencyObligation"/>
        <rdfs:comment xml:lang="it">Questa proprietà lega un argomento ad un obbligo di trasparenza.</rdfs:comment>
        <rdfs:comment xml:lang="en">This property links a subject to a transparency obligation.</rdfs:comment>
        <rdfs:isDefinedBy rdf:resource="https://w3id.org/italia/onto/Transparency/"/>
        <rdfs:label xml:lang="en">is object of an obligation</rdfs:label>
        <rdfs:label xml:lang="it">è oggetto di obbligo</rdfs:label>
    </owl:ObjectProperty>
    


    <!-- https://w3id.org/italia/onto/Transparency/isObligationContentOf -->

    <owl:ObjectProperty rdf:about="https://w3id.org/italia/onto/Transparency/isObligationContentOf">
        <rdfs:domain rdf:resource="https://w3id.org/italia/onto/Transparency/ObligationContent"/>
        <rdfs:range rdf:resource="https://w3id.org/italia/onto/Transparency/TransparencyObligation"/>
        <rdfs:comment xml:lang="it">Questa proprietà lega un obbligo di trasparenza ai suoi contenuti.</rdfs:comment>
        <rdfs:comment xml:lang="en">This property links a transparency obligation to its contents.</rdfs:comment>
        <rdfs:isDefinedBy rdf:resource="https://w3id.org/italia/onto/Transparency/"/>
        <rdfs:label xml:lang="en">if obligation content of</rdfs:label>
        <rdfs:label xml:lang="it">è contenuto obbligo di</rdfs:label>
    </owl:ObjectProperty>
    


    <!-- https://w3id.org/italia/onto/Transparency/publisher -->

    <owl:ObjectProperty rdf:about="https://w3id.org/italia/onto/Transparency/publisher">
        <owl:inverseOf rdf:resource="https://w3id.org/italia/onto/Transparency/publishes"/>
        <rdfs:domain rdf:resource="https://w3id.org/italia/onto/Transparency/Content"/>
        <rdfs:range rdf:resource="https://w3id.org/italia/onto/COV/PublicOrganization"/>
        <rdfs:comment xml:lang="it">Questa proprietà lega un contenuto alla pubblica amministrazione che lo pubblica.</rdfs:comment>
        <rdfs:comment xml:lang="en">This property links a content to the public administration that public it</rdfs:comment>
        <rdfs:isDefinedBy rdf:resource="https://w3id.org/italia/onto/Transparency/"/>
        <rdfs:label xml:lang="en">is published by</rdfs:label>
        <rdfs:label xml:lang="it">è pubblicato da</rdfs:label>
    </owl:ObjectProperty>
    


    <!-- https://w3id.org/italia/onto/Transparency/publishes -->

    <owl:ObjectProperty rdf:about="https://w3id.org/italia/onto/Transparency/publishes">
        <rdfs:domain rdf:resource="https://w3id.org/italia/onto/COV/PublicOrganization"/>
        <rdfs:range rdf:resource="https://w3id.org/italia/onto/Transparency/Content"/>
        <rdfs:comment xml:lang="it">Questa proprietà lega una pubblica amministrazione al contenuto che pubblica.</rdfs:comment>
        <rdfs:comment xml:lang="en">This property links a content to the public administration that public it</rdfs:comment>
        <rdfs:isDefinedBy rdf:resource="https://w3id.org/italia/onto/Transparency/"/>
        <rdfs:label xml:lang="it">pubblica</rdfs:label>
        <rdfs:label xml:lang="en">publishes</rdfs:label>
    </owl:ObjectProperty>
    


    <!-- https://w3id.org/italia/onto/Transparency/refersTo -->

    <owl:ObjectProperty rdf:about="https://w3id.org/italia/onto/Transparency/refersTo">
        <rdfs:domain rdf:resource="https://w3id.org/italia/onto/Transparency/TransparencySubject"/>
        <rdfs:range rdf:resource="http://www.w3.org/2002/07/owl#Thing"/>
        <rdfs:comment>Questa proprietà lega un argomento oggetto di obbligo di trasparenza all&apos;entità, eventualmente già modellata in OntoPiA, a cui si riferisce.</rdfs:comment>
        <rdfs:comment xml:lang="en">This property links a subject to a related entity, eventually already modelled by OntoPiA.</rdfs:comment>
        <rdfs:isDefinedBy rdf:resource="https://w3id.org/italia/onto/Transparency/"/>
        <rdfs:label xml:lang="en">refers to</rdfs:label>
        <rdfs:label xml:lang="it">si riferisce a</rdfs:label>
    </owl:ObjectProperty>
    


    <!-- 
    ///////////////////////////////////////////////////////////////////////////////////////
    //
    // Data properties
    //
    ///////////////////////////////////////////////////////////////////////////////////////
     -->

    


    <!-- https://w3id.org/italia/onto/SM/URL -->

    <owl:DatatypeProperty rdf:about="https://w3id.org/italia/onto/SM/URL">
        <owl:equivalentProperty rdf:resource="https://w3id.org/italia/onto/Transparency/sourceURL"/>
        <rdfs:isDefinedBy rdf:resource="https://w3id.org/italia/onto/SM/"/>
    </owl:DatatypeProperty>
    


    <!-- https://w3id.org/italia/onto/TI/issued -->

    <owl:DatatypeProperty rdf:about="https://w3id.org/italia/onto/TI/issued">
        <rdfs:isDefinedBy rdf:resource="https://w3id.org/italia/onto/TI/"/>
    </owl:DatatypeProperty>
    


    <!-- https://w3id.org/italia/onto/TI/modified -->

    <owl:DatatypeProperty rdf:about="https://w3id.org/italia/onto/TI/modified">
        <rdfs:isDefinedBy rdf:resource="https://w3id.org/italia/onto/TI/"/>
    </owl:DatatypeProperty>
    


    <!-- https://w3id.org/italia/onto/Transparency/regulationReference -->

    <owl:DatatypeProperty rdf:about="https://w3id.org/italia/onto/Transparency/regulationReference">
        <rdfs:domain>
            <owl:Class>
                <owl:unionOf rdf:parseType="Collection">
                    <rdf:Description rdf:about="https://w3id.org/italia/onto/Transparency/ObligationContent"/>
                    <rdf:Description rdf:about="https://w3id.org/italia/onto/Transparency/TransparencyObligation"/>
                </owl:unionOf>
            </owl:Class>
        </rdfs:domain>
        <rdfs:range rdf:resource="http://www.w3.org/2000/01/rdf-schema#Literal"/>
        <rdfs:comment xml:lang="en">regulation referred to the transparency obligation.</rdfs:comment>
        <rdfs:comment xml:lang="it">riferimento normativo all&apos;obbligo di pubblicazione.</rdfs:comment>
        <rdfs:isDefinedBy rdf:resource="https://w3id.org/italia/onto/Transparency/"/>
        <rdfs:label xml:lang="en">normative reference</rdfs:label>
        <rdfs:label xml:lang="it">riferimento normativo</rdfs:label>
    </owl:DatatypeProperty>
    


    <!-- https://w3id.org/italia/onto/Transparency/sourceURL -->

    <owl:DatatypeProperty rdf:about="https://w3id.org/italia/onto/Transparency/sourceURL">
        <rdfs:domain rdf:resource="https://w3id.org/italia/onto/Transparency/Content"/>
        <rdfs:range rdf:resource="http://www.w3.org/2001/XMLSchema#anyURI"/>
        <rdfs:comment xml:lang="it">Questa URL definisce l&apos;indirizzo di accesso e reperimento del contenuto informativo.</rdfs:comment>
        <rdfs:comment xml:lang="en">This URL defines the access address of the informative content.</rdfs:comment>
        <rdfs:isDefinedBy rdf:resource="https://w3id.org/italia/onto/Transparency/"/>
        <rdfs:label xml:lang="it">URL del contenuto</rdfs:label>
        <rdfs:label xml:lang="en">content URL</rdfs:label>
    </owl:DatatypeProperty>
    


    <!-- 
    ///////////////////////////////////////////////////////////////////////////////////////
    //
    // Classes
    //
    ///////////////////////////////////////////////////////////////////////////////////////
     -->

    


    <!-- http://dati.gov.it/onto/dcatapit#Agent -->

    <owl:Class rdf:about="http://dati.gov.it/onto/dcatapit#Agent"/>
    


    <!-- http://purl.org/dc/terms/Frequency -->

    <owl:Class rdf:about="http://purl.org/dc/terms/Frequency">
        <owl:equivalentClass rdf:resource="https://w3id.org/italia/onto/Transparency/Frequency"/>
    </owl:Class>
    


    <!-- http://xmlns.com/foaf/0.1/Agent -->

    <owl:Class rdf:about="http://xmlns.com/foaf/0.1/Agent"/>
    


    <!-- https://w3id.org/italia/onto/ADMS/SemanticAssetDistribution -->

    <owl:Class rdf:about="https://w3id.org/italia/onto/ADMS/SemanticAssetDistribution"/>
    


    <!-- https://w3id.org/italia/onto/COV/PublicOrganization -->

    <owl:Class rdf:about="https://w3id.org/italia/onto/COV/PublicOrganization">
        <rdfs:isDefinedBy rdf:resource="https://w3id.org/italia/onto/COV/"/>
        <rdfs:label xml:lang="it">Amministrazione pubblica</rdfs:label>
        <rdfs:label xml:lang="it">organizzazione pubblica</rdfs:label>
        <rdfs:label xml:lang="en">public organization</rdfs:label>
    </owl:Class>
    


    <!-- https://w3id.org/italia/onto/Transparency/Content -->

    <owl:Class rdf:about="https://w3id.org/italia/onto/Transparency/Content">
        <rdfs:subClassOf>
            <owl:Restriction>
                <owl:onProperty rdf:resource="https://w3id.org/italia/onto/Transparency/hasSubject"/>
                <owl:someValuesFrom rdf:resource="https://w3id.org/italia/onto/Transparency/TransparencySubject"/>
            </owl:Restriction>
        </rdfs:subClassOf>
        <rdfs:subClassOf>
            <owl:Restriction>
                <owl:onProperty rdf:resource="https://w3id.org/italia/onto/Transparency/publisher"/>
                <owl:allValuesFrom rdf:resource="https://w3id.org/italia/onto/COV/PublicOrganization"/>
            </owl:Restriction>
        </rdfs:subClassOf>
        <rdfs:subClassOf>
            <owl:Restriction>
                <owl:onProperty rdf:resource="https://w3id.org/italia/onto/Transparency/comply"/>
                <owl:minQualifiedCardinality rdf:datatype="http://www.w3.org/2001/XMLSchema#nonNegativeInteger">1</owl:minQualifiedCardinality>
                <owl:onClass rdf:resource="https://w3id.org/italia/onto/Transparency/ObligationContent"/>
            </owl:Restriction>
        </rdfs:subClassOf>
        <rdfs:subClassOf>
            <owl:Restriction>
                <owl:onProperty rdf:resource="https://w3id.org/italia/onto/TI/issued"/>
                <owl:qualifiedCardinality rdf:datatype="http://www.w3.org/2001/XMLSchema#nonNegativeInteger">1</owl:qualifiedCardinality>
                <owl:onDataRange>
                    <rdfs:Datatype>
                        <owl:unionOf rdf:parseType="Collection">
                            <rdf:Description rdf:about="http://www.w3.org/2001/XMLSchema#date"/>
                            <rdf:Description rdf:about="http://www.w3.org/2001/XMLSchema#dateTime"/>
                        </owl:unionOf>
                    </rdfs:Datatype>
                </owl:onDataRange>
            </owl:Restriction>
        </rdfs:subClassOf>
        <rdfs:subClassOf>
            <owl:Restriction>
                <owl:onProperty rdf:resource="https://w3id.org/italia/onto/TI/modified"/>
                <owl:qualifiedCardinality rdf:datatype="http://www.w3.org/2001/XMLSchema#nonNegativeInteger">1</owl:qualifiedCardinality>
                <owl:onDataRange>
                    <rdfs:Datatype>
                        <owl:unionOf rdf:parseType="Collection">
                            <rdf:Description rdf:about="http://www.w3.org/2001/XMLSchema#date"/>
                            <rdf:Description rdf:about="http://www.w3.org/2001/XMLSchema#dateTime"/>
                        </owl:unionOf>
                    </rdfs:Datatype>
                </owl:onDataRange>
            </owl:Restriction>
        </rdfs:subClassOf>
        <rdfs:subClassOf>
            <owl:Restriction>
                <owl:onProperty rdf:resource="https://w3id.org/italia/onto/Transparency/sourceURL"/>
                <owl:qualifiedCardinality rdf:datatype="http://www.w3.org/2001/XMLSchema#nonNegativeInteger">1</owl:qualifiedCardinality>
                <owl:onDataRange rdf:resource="http://www.w3.org/2001/XMLSchema#anyURI"/>
            </owl:Restriction>
        </rdfs:subClassOf>
        <rdfs:comment xml:lang="it">Questa classe rappresenta i documenti, le informazioni e i dati oggetto di pubblicazione nei siti istituzionali delle pubbliche amministrazioni.</rdfs:comment>
        <rdfs:comment xml:lang="en">This class represents documents, informazions and data object of publication on the official website of the public administrations.</rdfs:comment>
        <rdfs:isDefinedBy rdf:resource="https://w3id.org/italia/onto/Transparency/"/>
        <rdfs:label xml:lang="en">Content</rdfs:label>
        <rdfs:label xml:lang="it">Contenuto</rdfs:label>
    </owl:Class>
    


    <!-- https://w3id.org/italia/onto/Transparency/Frequency -->

    <owl:Class rdf:about="https://w3id.org/italia/onto/Transparency/Frequency">
        <rdfs:comment xml:lang="en">A rate at which something recurs. It is used to represent the frequency of update of published informative content. It assumes a specific set of values as defined by the controlled vocabulary available at http://publications.europa.eu/mdr/authority/frequency/index.html. The class is equivalent to the class defined by the Dublin Core standard</rdfs:comment>
        <rdfs:comment xml:lang="it">Numero delle volte che qualcosa si ripete. E&apos; utlizzata per rappresentare la frequenza di aggiornamento del contenuto informativo pubblicato come specificato nella norma di riferimento. Essa assume un insieme finito di valori come definiti dal vocabolario controllato disponibile in http://publications.europa.eu/mdr/authority/frequency/index.html. La classe è equivalente alla classe dallo standard dublin core</rdfs:comment>
        <rdfs:isDefinedBy rdf:resource="https://w3id.org/italia/onto/Transparency/"/>
        <rdfs:label xml:lang="en">Frequency</rdfs:label>
        <rdfs:label xml:lang="it">Frequenza</rdfs:label>
    </owl:Class>
    


    <!-- https://w3id.org/italia/onto/Transparency/ObligationContent -->

    <owl:Class rdf:about="https://w3id.org/italia/onto/Transparency/ObligationContent">
        <rdfs:subClassOf>
            <owl:Restriction>
                <owl:onProperty rdf:resource="https://w3id.org/italia/onto/Transparency/accrualPeriodicity"/>
                <owl:qualifiedCardinality rdf:datatype="http://www.w3.org/2001/XMLSchema#nonNegativeInteger">1</owl:qualifiedCardinality>
                <owl:onClass rdf:resource="https://w3id.org/italia/onto/Transparency/Frequency"/>
            </owl:Restriction>
        </rdfs:subClassOf>
        <rdfs:subClassOf>
            <owl:Restriction>
                <owl:onProperty rdf:resource="https://w3id.org/italia/onto/Transparency/isObligationContentOf"/>
                <owl:qualifiedCardinality rdf:datatype="http://www.w3.org/2001/XMLSchema#nonNegativeInteger">1</owl:qualifiedCardinality>
                <owl:onClass rdf:resource="https://w3id.org/italia/onto/Transparency/TransparencyObligation"/>
            </owl:Restriction>
        </rdfs:subClassOf>
        <rdfs:subClassOf>
            <owl:Restriction>
                <owl:onProperty rdf:resource="https://w3id.org/italia/onto/Transparency/regulationReference"/>
                <owl:cardinality rdf:datatype="http://www.w3.org/2001/XMLSchema#nonNegativeInteger">1</owl:cardinality>
            </owl:Restriction>
        </rdfs:subClassOf>
        <rdfs:comment>Questa classe rappresenta il contenuto informativo riferito ad un obbligo di trasparenza oggetto di pubblicazione. Fa riferimento alla colonna &apos;contenuto dell&apos;obbligo&apos; dell&apos;allegato alla guida ANAC. </rdfs:comment>
        <rdfs:comment xml:lang="en">This class represents the informative content referred to a transparency obligation. It&apos;s related to the &apos;contenuto dell&apos;obbligo&apos; column of the ANAC guideline attachment.</rdfs:comment>
        <rdfs:isDefinedBy rdf:resource="https://w3id.org/italia/onto/Transparency/"/>
        <rdfs:label xml:lang="en">Content of the obligation</rdfs:label>
        <rdfs:label xml:lang="it">Contenuto dell&apos;obbligo</rdfs:label>
    </owl:Class>
    


    <!-- https://w3id.org/italia/onto/Transparency/TransparencyObligation -->

    <owl:Class rdf:about="https://w3id.org/italia/onto/Transparency/TransparencyObligation">
        <rdfs:subClassOf>
            <owl:Restriction>
                <owl:onProperty rdf:resource="https://w3id.org/italia/onto/Transparency/affects"/>
                <owl:allValuesFrom rdf:resource="https://w3id.org/italia/onto/Transparency/TransparencySubject"/>
            </owl:Restriction>
        </rdfs:subClassOf>
        <rdfs:subClassOf>
            <owl:Restriction>
                <owl:onProperty rdf:resource="https://w3id.org/italia/onto/Transparency/isAppliedTo"/>
                <owl:allValuesFrom rdf:resource="https://w3id.org/italia/onto/COV/PublicOrganization"/>
            </owl:Restriction>
        </rdfs:subClassOf>
        <rdfs:subClassOf>
            <owl:Restriction>
                <owl:onProperty rdf:resource="https://w3id.org/italia/onto/Transparency/hasObligationContent"/>
                <owl:minQualifiedCardinality rdf:datatype="http://www.w3.org/2001/XMLSchema#nonNegativeInteger">1</owl:minQualifiedCardinality>
                <owl:onClass rdf:resource="https://w3id.org/italia/onto/Transparency/ObligationContent"/>
            </owl:Restriction>
        </rdfs:subClassOf>
        <rdfs:subClassOf>
            <owl:Restriction>
                <owl:onProperty rdf:resource="https://w3id.org/italia/onto/Transparency/hasTransparencySubSection"/>
                <owl:qualifiedCardinality rdf:datatype="http://www.w3.org/2001/XMLSchema#nonNegativeInteger">1</owl:qualifiedCardinality>
                <owl:onClass rdf:resource="https://w3id.org/italia/onto/Transparency/TransparencyTitulus"/>
            </owl:Restriction>
        </rdfs:subClassOf>
        <rdfs:subClassOf>
            <owl:Restriction>
                <owl:onProperty rdf:resource="https://w3id.org/italia/onto/Transparency/regulationReference"/>
                <owl:cardinality rdf:datatype="http://www.w3.org/2001/XMLSchema#nonNegativeInteger">1</owl:cardinality>
            </owl:Restriction>
        </rdfs:subClassOf>
        <rdfs:comment xml:lang="it">Questa classe rappresenta gli argomenti oggetto di obbligo di pubblicazione per la normativa sulla trasparenza. Fa riferimento alla colonna &apos;denominazione obbligo&apos; dell&apos;allegato alla guida ANAC.</rdfs:comment>
        <rdfs:comment xml:lang="en">This class represents the topic object of transparency obligation according to the transparency normative. It&apos;s related to the &apos;denominazione obbligo&apos; column of the ANAC guideline attachment.</rdfs:comment>
        <rdfs:isDefinedBy rdf:resource="https://w3id.org/italia/onto/Transparency/"/>
        <rdfs:label xml:lang="it">Obbligo di trasparenza</rdfs:label>
        <rdfs:label xml:lang="en">Obligation of transparency</rdfs:label>
    </owl:Class>
    


    <!-- https://w3id.org/italia/onto/Transparency/TransparencySubject -->

    <owl:Class rdf:about="https://w3id.org/italia/onto/Transparency/TransparencySubject">
        <rdfs:subClassOf rdf:resource="https://w3id.org/italia/onto/l0/Entity"/>
        <rdfs:subClassOf>
            <owl:Restriction>
                <owl:onProperty rdf:resource="https://w3id.org/italia/onto/Transparency/hasContent"/>
                <owl:someValuesFrom rdf:resource="https://w3id.org/italia/onto/Transparency/Content"/>
            </owl:Restriction>
        </rdfs:subClassOf>
        <rdfs:subClassOf>
            <owl:Restriction>
                <owl:onProperty rdf:resource="https://w3id.org/italia/onto/Transparency/isObjectOfObligation"/>
                <owl:someValuesFrom rdf:resource="https://w3id.org/italia/onto/Transparency/TransparencyObligation"/>
            </owl:Restriction>
        </rdfs:subClassOf>
        <rdfs:comment xml:lang="it">Questa classe rappresenta il soggetto a cui fa riferimento il contenuto da pubblicare.</rdfs:comment>
        <rdfs:comment xml:lang="en">This class represents the subject related to the content to publish</rdfs:comment>
        <rdfs:isDefinedBy rdf:resource="https://w3id.org/italia/onto/Transparency/"/>
        <rdfs:label xml:lang="it">Soggetto del contenuto della trasparenza</rdfs:label>
        <rdfs:label xml:lang="en">Subject of transparency contents</rdfs:label>
    </owl:Class>
    


    <!-- https://w3id.org/italia/onto/Transparency/TransparencyTitulus -->

    <owl:Class rdf:about="https://w3id.org/italia/onto/Transparency/TransparencyTitulus">
        <rdfs:comment xml:lang="it">Questa classe la denominazione delle sotto-sezioni della sezione &apos;Amministrazione Trasparente&apos; del sito istituzionale delle pubbliche amministrazioni. Le voci sono controllate dal vocabolario &lt;https://w3id.org/italia/controlled-vocabulary/classifications-for-transparency/transparency-titulus&gt;.</rdfs:comment>
        <rdfs:comment xml:lang="en">This class represents the subsections of the &apos;Transaprent Administrazion&apos; section of the official website of the public administrations. The individuals are controlled by the vocabulary &lt;https://w3id.org/italia/controlled-vocabulary/classifications-for-transparency/transparency-titulus&gt;.</rdfs:comment>
        <rdfs:isDefinedBy rdf:resource="https://w3id.org/italia/onto/Transparency/"/>
        <rdfs:label xml:lang="it">Denominazione sotto-sezione Amministrazione Trasparente</rdfs:label>
        <rdfs:label xml:lang="en">Transparent administration sub-section denomination</rdfs:label>
        <l0:controlledVocabulary rdf:resource="https://w3id.org/italia/controlled-vocabulary/classifications-for-transparency/transparency-titulus"/>
    </owl:Class>
    


    <!-- https://w3id.org/italia/onto/l0/Entity -->

    <owl:Class rdf:about="https://w3id.org/italia/onto/l0/Entity">
        <rdfs:isDefinedBy rdf:resource="https://w3id.org/italia/onto/l0/"/>
    </owl:Class>
    


    <!-- 
    ///////////////////////////////////////////////////////////////////////////////////////
    //
    // Individuals
    //
    ///////////////////////////////////////////////////////////////////////////////////////
     -->

    


    <!-- http://spcdata.digitpa.gov.it/Amministrazione/agid -->

    <owl:NamedIndividual rdf:about="http://spcdata.digitpa.gov.it/Amministrazione/agid">
        <rdf:type rdf:resource="http://dati.gov.it/onto/dcatapit#Agent"/>
        <rdf:type rdf:resource="http://xmlns.com/foaf/0.1/Agent"/>
        <dct:identifier>agid</dct:identifier>
        <foaf:name xml:lang="it">Agenzia per l&apos;Italia Digitale</foaf:name>
        <foaf:name xml:lang="en">Italian Digital Agency</foaf:name>
    </owl:NamedIndividual>
    


    <!-- https://w3id.org/italia/data/distribution/TRAPIT-JSON-LD -->

    <owl:NamedIndividual rdf:about="https://w3id.org/italia/data/distribution/TRAPIT-JSON-LD">
        <rdf:type rdf:resource="https://w3id.org/italia/onto/ADMS/SemanticAssetDistribution"/>
        <dct:description xml:lang="it">Questa è la distribuzione JSON-LD dell&apos;ontologia dell&apos;amministrazione trasparente</dct:description>
        <dct:description xml:lang="en">This is the distribution in JSON-LD of the transparent administration</dct:description>
        <dct:format rdf:resource="http://publications.europa.eu/resource/authority/file-type/JSON_LD"/>
        <dct:license rdf:resource="https://w3id.org/italia/controlled-vocabulary/licences/A21_CCBY40"/>
        <dct:title xml:lang="it">Distribuzione JSON-LD ontologia Transparency-AP_IT</dct:title>
        <dct:title xml:lang="en">JSON-LD distribution of Transparency-AP_IT Ontology</dct:title>
        <dcat:accessURL rdf:resource="https://raw.githubusercontent.com/italia/daf-ontologie-vocabolari-controllati/master/Ontologie/Transparency/latest"/>
        <dcat:downloadURL rdf:resource="https://raw.githubusercontent.com/italia/daf-ontologie-vocabolari-controllati/master/Ontologie/Transparency/Transparency-AP_IT.jsonld"/>
    </owl:NamedIndividual>
    


    <!-- https://w3id.org/italia/data/distribution/TRAPIT-RDF-TURTLE -->

    <owl:NamedIndividual rdf:about="https://w3id.org/italia/data/distribution/TRAPIT-RDF-TURTLE">
        <rdf:type rdf:resource="https://w3id.org/italia/onto/ADMS/SemanticAssetDistribution"/>
        <dct:description xml:lang="it">Questa è la distribuzione RDF/Turtle dell&apos;ontologia dell&apos;amministrazione trasparente</dct:description>
        <dct:description xml:lang="en">This is the distribution in RDF/Turtle of the transparent administration</dct:description>
        <dct:format rdf:resource="http://publications.europa.eu/resource/authority/file-type/RDF_TURTLE"/>
        <dct:license rdf:resource="https://w3id.org/italia/controlled-vocabulary/licences/A21_CCBY40"/>
        <dct:title xml:lang="it">Distribuzione RDF/Turtle ontologia Transparency-AP_IT</dct:title>
        <dct:title xml:lang="en">RDF/Turtle distribution of Transparency-AP_IT Ontology</dct:title>
        <dcat:accessURL rdf:resource="https://raw.githubusercontent.com/italia/daf-ontologie-vocabolari-controllati/master/Ontologie/Transparency/latest"/>
        <dcat:downloadURL rdf:resource="https://raw.githubusercontent.com/italia/daf-ontologie-vocabolari-controllati/master/Ontologie/Transparency/Transparency-AP_IT.ttl"/>
    </owl:NamedIndividual>
    


    <!-- https://w3id.org/italia/data/distribution/TRAPIT-RDF-XML -->

    <owl:NamedIndividual rdf:about="https://w3id.org/italia/data/distribution/TRAPIT-RDF-XML">
        <rdf:type rdf:resource="https://w3id.org/italia/onto/ADMS/SemanticAssetDistribution"/>
        <dct:description xml:lang="it">Questa è la distribuzione RDF/XML dell&apos;ontologia dell&apos;amministrazione trasparente</dct:description>
        <dct:description xml:lang="en">This is the distribution in RDF/XML of the transparent administration</dct:description>
        <dct:format rdf:resource="http://publications.europa.eu/resource/authority/file-type/RDF_XML"/>
        <dct:license rdf:resource="https://w3id.org/italia/controlled-vocabulary/licences/A21_CCBY40"/>
        <dct:title xml:lang="it">Distribuzione RDF/XML ontologia Transparency-AP_IT</dct:title>
        <dct:title xml:lang="en">RDF/XML distribution of Transparency-AP_IT Ontology</dct:title>
        <dcat:accessURL rdf:resource="https://raw.githubusercontent.com/italia/daf-ontologie-vocabolari-controllati/master/Ontologie/Transparency/latest"/>
        <dcat:downloadURL rdf:resource="https://raw.githubusercontent.com/italia/daf-ontologie-vocabolari-controllati/master/Ontologie/Transparency/Transparency-AP_IT.rdf"/>
    </owl:NamedIndividual>
    


    <!-- https://w3id.org/italia/data/organization/private-organization/05481840964 -->

    <owl:NamedIndividual rdf:about="https://w3id.org/italia/data/organization/private-organization/05481840964">
        <rdf:type rdf:resource="http://dati.gov.it/onto/dcatapit#Agent"/>
        <rdf:type rdf:resource="http://xmlns.com/foaf/0.1/Agent"/>
        <dct:identifier>05481840964</dct:identifier>
        <foaf:name xml:lang="it">Almawave Srl</foaf:name>
    </owl:NamedIndividual>
</rdf:RDF>



<!-- Generated by the OWL API (version 4.2.8.20170104-2310) https://github.com/owlcs/owlapi -->

