<?xml version="1.0"?>
<rdf:RDF xmlns="https://w3id.org/italia/onto/Transparency#"
     xml:base="https://w3id.org/italia/onto/Transparency"
     xmlns:dc="http://purl.org/dc/elements/1.1/"
     xmlns:l0="https://w3id.org/italia/onto/l0/"
     xmlns:dct="http://purl.org/dc/terms/"
     xmlns:owl="http://www.w3.org/2002/07/owl#"
     xmlns:rdf="http://www.w3.org/1999/02/22-rdf-syntax-ns#"
     xmlns:xml="http://www.w3.org/XML/1998/namespace"
     xmlns:xsd="http://www.w3.org/2001/XMLSchema#"
     xmlns:adms="http://www.w3.org/ns/adms#"
     xmlns:dcat="http://www.w3.org/ns/dcat#"
     xmlns:foaf="http://xmlns.com/foaf/0.1/"
     xmlns:prov="http://www.w3.org/ns/prov#"
     xmlns:rdfs="http://www.w3.org/2000/01/rdf-schema#"
     xmlns:skos="http://www.w3.org/2004/02/skos/core#"
     xmlns:xkos="http://rdf-vocabulary.ddialliance.org/xkos#"
     xmlns:vcard="http://www.w3.org/2006/vcard/ns#"
     xmlns:smapit="https://w3id.org/italia/onto/SM/"
     xmlns:tiapit="https://w3id.org/italia/onto/TI/"
     xmlns:clvapit="https://w3id.org/italia/onto/CLV/"
     xmlns:covapit="https://w3id.org/italia/onto/COV/"
     xmlns:admsapit="https://w3id.org/italia/onto/ADMS/"
     xmlns:cpsvapit="https://w3id.org/italia/onto/CPSV/"
     xmlns:dcatapit="http://dati.gov.it/onto/dcatapit#">
    <owl:Ontology rdf:about="https://w3id.org/italia/onto/Transparency">
        <owl:versionIRI rdf:resource="https://w3id.org/italia/onto/Transparency/0.1"/>
        <owl:imports rdf:resource="https://w3id.org/italia/onto/COV"/>
        <owl:imports rdf:resource="https://w3id.org/italia/onto/TI"/>
        <owl:imports rdf:resource="https://w3id.org/italia/onto/l0"/>
        <dct:accrualPeriodicity rdf:resource="http://publications.europa.eu/resource/authority/frequency/IRREG"/>
        <dct:creator rdf:resource="http://spcdata.digitpa.gov.it/Amministrazione/agid"/>
        <dct:creator rdf:resource="https://w3id.org/italia/data/organization/private-organization/05481840964"/>
        <dct:description rdf:resource="https://w3id.org/italia/onto/Transparency/./latest/img/Transparency-AP_IT.png"/>
        <dct:description>Questa versione dell&apos;ontologia è in attesa di essere visionata da ANAC.@it</dct:description>
        <dct:description xml:lang="it">Questo è il profilo applicativo italiano dell&apos;ontologia sull&apos;amministrazione trasparente. L&apos;ontologia di OntoPiA implementa le disposizioni in merito all&apos;obbligo di pubblicazione di contenuti informativi nella sezione &apos;Amministrazione Trasparente&apos; dei siti istituzioonali delle publiche amministrazioni.</dct:description>
        <dct:description xml:lang="en">This is the Italian application profile of the ontology on the transparent administration. This ontology of OntoPiA implements the dispositions about the publication obligation of informative contents on the section &apos;Transparent Administration&apos; of the official website of the public administrations.</dct:description>
        <dct:description xml:lang="en">This ontology version is a draft waiting for the ANAC validation.</dct:description>
        <dct:issued rdf:datatype="http://www.w3.org/2001/XMLSchema#date">2019-05-29</dct:issued>
        <dct:language rdf:resource="http://publications.europa.eu/resource/authority/language/ENG"/>
        <dct:language rdf:resource="http://publications.europa.eu/resource/authority/language/ITA"/>
        <dct:modified rdf:datatype="http://www.w3.org/2001/XMLSchema#date">2019-03-04</dct:modified>
        <dct:publisher rdf:resource="http://spcdata.digitpa.gov.it/Amministrazione/agid"/>
        <dct:rightsHolder rdf:resource="http://spcdata.digitpa.gov.it/Amministrazione/agid"/>
        <dct:title xml:lang="it">Ontologia dell&apos;Amministrazione Trasparente - profilo applicativo italiano</dct:title>
        <rdfs:comment>Questa versione dell&apos;ontologia è in attesa di essere visionata da ANAC.@it</rdfs:comment>
        <rdfs:comment xml:lang="it">Questo è il profilo applicativo italiano dell&apos;ontologia sull&apos;amministrazione trasparente. L&apos;ontologia di OntoPiA implementa le disposizioni in merito all&apos;obbligo di pubblicazione di contenuti informativi nella sezione &apos;Amministrazione Trasparente&apos; dei siti istituzionali delle publiche amministrazioni.</rdfs:comment>
        <rdfs:comment xml:lang="en">This is the Italian application profile of the ontology on the transparent administration. This ontology of OntoPiA implements the dispositions about the publication obligation of informative contents on the section &apos;Transparent Administration&apos; of the official website of the public administrations.</rdfs:comment>
        <rdfs:comment xml:lang="en">This ontology version is a draft waiting for the ANAC validation.</rdfs:comment>
        <rdfs:isDefinedBy rdf:resource="https://w3id.org/italia/onto/Transparency"/>
        <rdfs:label xml:lang="it">Ontologia dell&apos;Amministrazione Trasparente - profilo applicativo italiano</rdfs:label>
        <rdfs:label xml:lang="en">Transparent Administration Ontology - Italian application profile</rdfs:label>
        <owl:versionInfo xml:lang="it">La presente versione dell&apos;ontologia è un draft in attesa di revisone da parte di ANAC.</owl:versionInfo>
        <dcat:contactPoint rdf:resource="http://dati.gov.it/data/resource/ContactPoint/voc_AgID"/>
        <dcat:keyword xml:lang="en">transparency</dcat:keyword>
        <dcat:keyword xml:lang="en">transparency for public administration</dcat:keyword>
        <dcat:keyword xml:lang="it">trasparenza</dcat:keyword>
        <dcat:keyword xml:lang="it">trasparenza PA</dcat:keyword>
        <dcat:keyword xml:lang="it">trasparenza pa</dcat:keyword>
        <dcat:keyword xml:lang="it">trasparenza pubblica amministrazione</dcat:keyword>
        <dcat:theme rdf:resource="http://publications.europa.eu/resource/authority/data-theme/GOVE"/>
        <dcat:theme rdf:resource="http://publications.europa.eu/resource/authority/data-theme/TECH"/>
        <admsapit:acronym>Transparency-AP_IT</admsapit:acronym>
        <admsapit:hasFormalityLevel rdf:resource="https://w3id.org/italia/onto/ADMS/Formal"/>
        <admsapit:hasOntologyLanguage rdf:resource="https://w3id.org/italia/onto/ADMS/OWL"/>
        <admsapit:hasSemanticAssetDistribution rdf:resource="https://w3id.org/italia/data/distribution/TRAPIT-JSON-LD"/>
        <admsapit:hasSemanticAssetDistribution rdf:resource="https://w3id.org/italia/data/distribution/TRAPIT-RDF-TURTLE"/>
        <admsapit:hasSemanticAssetDistribution rdf:resource="https://w3id.org/italia/data/distribution/TRAPIT-RDF-XML"/>
        <admsapit:hasTask rdf:resource="https://w3id.org/italia/onto/ADMS/AnnotationTask"/>
        <admsapit:hasTask rdf:resource="https://w3id.org/italia/onto/ADMS/QueryFormulationTask"/>
        <admsapit:hasTask rdf:resource="https://w3id.org/italia/onto/ADMS/SearchTask"/>
        <admsapit:last rdf:resource="https://w3id.org/italia/onto/Transparency/0.1"/>
        <admsapit:officialURI rdf:datatype="http://www.w3.org/2001/XMLSchema#anyURI">https://w3id.org/italia/onto/Transparency</admsapit:officialURI>
        <admsapit:prefix>trapit</admsapit:prefix>
        <admsapit:semanticAssetInUse rdf:resource="https://w3id.org/italia/data/project/DAF"/>
        <admsapit:semanticAssetInUse rdf:resource="https://w3id.org/italia/data/project/OntoPiA"/>
        <admsapit:status>draft</admsapit:status>
        <admsapit:target xml:lang="it">Cittadini</admsapit:target>
        <admsapit:target xml:lang="it">Pubbliche amministrazioni</admsapit:target>
        <admsapit:type rdf:resource="https://w3id.org/italia/onto/ADMS/DomainOntology"/>
    </owl:Ontology>
    


    <!-- 
    ///////////////////////////////////////////////////////////////////////////////////////
    //
    // Annotation properties
    //
    ///////////////////////////////////////////////////////////////////////////////////////
     -->

    


    <!-- http://www.w3.org/2000/01/rdf-schema#labels -->

    <owl:AnnotationProperty rdf:about="http://www.w3.org/2000/01/rdf-schema#labels"/>
    


    <!-- 
    ///////////////////////////////////////////////////////////////////////////////////////
    //
    // Datatypes
    //
    ///////////////////////////////////////////////////////////////////////////////////////
     -->

    


    <!-- http://www.w3.org/2001/XMLSchema#date -->

    <rdfs:Datatype rdf:about="http://www.w3.org/2001/XMLSchema#date"/>
    


    <!-- http://www.w3.org/2001/XMLSchema#time -->

    <rdfs:Datatype rdf:about="http://www.w3.org/2001/XMLSchema#time"/>
    


    <!-- 
    ///////////////////////////////////////////////////////////////////////////////////////
    //
    // Object Properties
    //
    ///////////////////////////////////////////////////////////////////////////////////////
     -->

    


    <!-- https://w3id.org/italia/onto/Transparency/appliesToPA -->

    <owl:ObjectProperty rdf:about="https://w3id.org/italia/onto/Transparency/appliesToPA">
        <owl:inverseOf rdf:resource="https://w3id.org/italia/onto/Transparency/obligedToEnforce"/>
        <rdfs:domain rdf:resource="https://w3id.org/italia/onto/Transparency/TransparencyObligation"/>
        <rdfs:range rdf:resource="https://w3id.org/italia/onto/COV/PublicOrganization"/>
        <rdfs:comment xml:lang="it">Questa proprietà lega un obbligo di trasparenza alla pubblica amministrazione a cui si applica.</rdfs:comment>
        <rdfs:comment xml:lang="en">This property links a transparency obligation to a public administration to whom is applied.</rdfs:comment>
        <rdfs:isDefinedBy rdf:resource="https://w3id.org/italia/onto/Transparency"/>
        <rdfs:label xml:lang="en">applies to PA</rdfs:label>
        <rdfs:label xml:lang="it">si applica alla PA</rdfs:label>
    </owl:ObjectProperty>
    


    <!-- https://w3id.org/italia/onto/Transparency/definesUpdateFrequency -->

    <owl:ObjectProperty rdf:about="https://w3id.org/italia/onto/Transparency/definesUpdateFrequency">
        <rdfs:domain rdf:resource="https://w3id.org/italia/onto/Transparency/TransparencyObligation"/>
        <rdfs:range rdf:resource="https://w3id.org/italia/onto/Transparency/UpdateFrequency"/>
        <rdfs:comment xml:lang="it">Questa proprietà collega un obbligo di trasparenza alla frequenza di aggiornamento da esso definita.</rdfs:comment>
        <rdfs:comment xml:lang="en">This property links a transparency obligation to the update frequency which it defines.</rdfs:comment>
        <rdfs:isDefinedBy rdf:resource="https://w3id.org/italia/onto/Transparency"/>
        <rdfs:label xml:lang="en">defines update frequency</rdfs:label>
        <rdfs:label xml:lang="it">definisce frequenza di aggiornamento</rdfs:label>
    </owl:ObjectProperty>
    


    <!-- https://w3id.org/italia/onto/Transparency/generatedBy -->

    <owl:ObjectProperty rdf:about="https://w3id.org/italia/onto/Transparency/generatedBy">
        <owl:inverseOf rdf:resource="https://w3id.org/italia/onto/Transparency/generatesResource"/>
        <rdfs:domain rdf:resource="https://w3id.org/italia/onto/Transparency/TransparencyResource"/>
        <rdfs:range rdf:resource="https://w3id.org/italia/onto/Transparency/TransparencyActivity"/>
        <rdfs:comment xml:lang="it">Questa proprità lega una risorsa all&apos;attività che la genera.</rdfs:comment>
        <rdfs:comment xml:lang="en">This property links a transparency resource to the activity from which is generated by.</rdfs:comment>
        <rdfs:isDefinedBy rdf:resource="https://w3id.org/italia/onto/Transparency"/>
        <rdfs:label xml:lang="en">generated by</rdfs:label>
        <rdfs:label xml:lang="it">generato da</rdfs:label>
    </owl:ObjectProperty>
    


    <!-- https://w3id.org/italia/onto/Transparency/generatesResource -->

    <owl:ObjectProperty rdf:about="https://w3id.org/italia/onto/Transparency/generatesResource">
        <rdfs:domain rdf:resource="https://w3id.org/italia/onto/Transparency/TransparencyActivity"/>
        <rdfs:range rdf:resource="https://w3id.org/italia/onto/Transparency/TransparencyResource"/>
        <rdfs:comment xml:lang="it">Questa proprietà lega un&apos;attività della trasparenza alla risorsa generata come risultato dell&apos;attività.</rdfs:comment>
        <rdfs:comment xml:lang="en">This property links a transparency activity to the resource generated as outcome of it.</rdfs:comment>
        <rdfs:isDefinedBy rdf:resource="https://w3id.org/italia/onto/Transparency"/>
        <rdfs:label xml:lang="en">generates resource</rdfs:label>
        <rdfs:label xml:lang="it">produce risorsa</rdfs:label>
    </owl:ObjectProperty>
    


    <!-- https://w3id.org/italia/onto/Transparency/hasAllowedFormat -->

    <owl:ObjectProperty rdf:about="https://w3id.org/italia/onto/Transparency/hasAllowedFormat">
        <rdfs:domain rdf:resource="https://w3id.org/italia/onto/Transparency/TransparencyResource"/>
        <rdfs:range rdf:resource="https://w3id.org/italia/onto/Transparency/Format"/>
        <rdfs:comment xml:lang="it">Questa proprità lega una risorsa della trasparenza al formato definito per la pubblicazione</rdfs:comment>
        <rdfs:comment xml:lang="en">This property links a transparency resource to the allowed format defined for publication.</rdfs:comment>
        <rdfs:isDefinedBy rdf:resource="https://w3id.org/italia/onto/Transparency"/>
        <rdfs:label xml:lang="it">da pubblicare nel formato</rdfs:label>
        <rdfs:label xml:lang="en">has allowed format</rdfs:label>
    </owl:ObjectProperty>
    


    <!-- https://w3id.org/italia/onto/Transparency/hasTransparencyActivityTypology -->

    <owl:ObjectProperty rdf:about="https://w3id.org/italia/onto/Transparency/hasTransparencyActivityTypology">
        <rdfs:domain rdf:resource="https://w3id.org/italia/onto/Transparency/TransparencyActivity"/>
        <rdfs:range rdf:resource="https://w3id.org/italia/onto/Transparency/TransparencyActivityTypology"/>
        <rdfs:comment xml:lang="it">Questa proprietà lega una attività della trasparenza alla sua tipologia.</rdfs:comment>
        <rdfs:comment xml:lang="en">This property links a transparency activity to its typology.</rdfs:comment>
        <rdfs:isDefinedBy rdf:resource="https://w3id.org/italia/onto/Transparency"/>
        <rdfs:label xml:lang="it">ha tipologia di attività della trasparenza</rdfs:label>
        <rdfs:label xml:lang="en">has transparency activity typology</rdfs:label>
    </owl:ObjectProperty>
    


    <!-- https://w3id.org/italia/onto/Transparency/hasTransparencyStatus -->

    <owl:ObjectProperty rdf:about="https://w3id.org/italia/onto/Transparency/hasTransparencyStatus">
        <rdfs:domain rdf:resource="https://w3id.org/italia/onto/Transparency/TransparencyObligation"/>
        <rdfs:range rdf:resource="https://w3id.org/italia/onto/Transparency/TransparencyObligationStatus"/>
        <rdfs:comment xml:lang="it">Questa proprietà lega un obbligo di trasparenza al suo stato attuale.</rdfs:comment>
        <rdfs:comment xml:lang="en">This property links a transparency obligation to its current status.</rdfs:comment>
        <rdfs:isDefinedBy rdf:resource="https://w3id.org/italia/onto/Transparency"/>
        <rdfs:label xml:lang="it">ha stato</rdfs:label>
        <rdfs:label xml:lang="en">has transparency status</rdfs:label>
    </owl:ObjectProperty>
    


    <!-- https://w3id.org/italia/onto/Transparency/hasTransparencySubject -->

    <owl:ObjectProperty rdf:about="https://w3id.org/italia/onto/Transparency/hasTransparencySubject">
        <rdfs:domain rdf:resource="https://w3id.org/italia/onto/Transparency/TransparencyObligation"/>
        <rdfs:range rdf:resource="https://w3id.org/italia/onto/Transparency/TransparencySubject"/>
        <rdfs:comment xml:lang="it">Questa proprietà lega un obbligo di trasparenza ai temi che lo caratterizzano.</rdfs:comment>
        <rdfs:comment xml:lang="en">This property links a transparency obligation to the related subjects.</rdfs:comment>
        <rdfs:isDefinedBy rdf:resource="https://w3id.org/italia/onto/Transparency"/>
        <rdfs:label xml:lang="it">ha soggetto della trasparenza</rdfs:label>
        <rdfs:label xml:lang="it">ha tema della trasparenza</rdfs:label>
        <rdfs:label xml:lang="en">has transparency subject</rdfs:label>
        <rdfs:label xml:lang="en">has transparency theme</rdfs:label>
    </owl:ObjectProperty>
    


    <!-- https://w3id.org/italia/onto/Transparency/isClassifiedBy -->

    <owl:ObjectProperty rdf:about="https://w3id.org/italia/onto/Transparency/isClassifiedBy">
        <rdfs:domain rdf:resource="https://w3id.org/italia/onto/Transparency/TransparencyObligation"/>
        <rdfs:range rdf:resource="https://w3id.org/italia/onto/Transparency/TransparencyDataTypology"/>
        <rdfs:comment xml:lang="it">Questa proprietà lega un obbligo di trasparenza alla relativa tipologia. Le voci sono controllate della tassonomia https://w3id.org/italia/controlled-vocabulary/classifications-for-transparency/transparency-titulus</rdfs:comment>
        <rdfs:comment xml:lang="en">This property links a transparency obligation to the corresponding data typology. The values are controlled by the taxonomy  https://w3id.org/italia/controlled-vocabulary/classifications-for-transparency/transparency-titulus </rdfs:comment>
        <rdfs:isDefinedBy rdf:resource="https://w3id.org/italia/onto/Transparency"/>
        <rdfs:labels xml:lang="en">is calssified by</rdfs:labels>
        <rdfs:labels xml:lang="it">è classificato da</rdfs:labels>
    </owl:ObjectProperty>
    


    <!-- https://w3id.org/italia/onto/Transparency/isComposedByObligation -->

    <owl:ObjectProperty rdf:about="https://w3id.org/italia/onto/Transparency/isComposedByObligation">
        <owl:inverseOf rdf:resource="https://w3id.org/italia/onto/Transparency/isComposedByObligation"/>
        <owl:inverseOf rdf:resource="https://w3id.org/italia/onto/Transparency/isPartOfObligation"/>
        <rdfs:domain rdf:resource="https://w3id.org/italia/onto/Transparency/TransparencyObligation"/>
        <rdfs:range rdf:resource="https://w3id.org/italia/onto/Transparency/TransparencyObligation"/>
        <rdfs:comment xml:lang="it">Questa proprietà lega un obbligo di trasparenza ad obblighi di trasparenza più specifici.</rdfs:comment>
        <rdfs:comment xml:lang="en">This property links a transparency obligation to less general trasparency obligations.</rdfs:comment>
        <rdfs:isDefinedBy rdf:resource="https://w3id.org/italia/onto/Transparency"/>
        <rdfs:label xml:lang="en">is composed by transparency obligation</rdfs:label>
        <rdfs:label xml:lang="it">è composto da obbligo di trasparenza</rdfs:label>
    </owl:ObjectProperty>
    


    <!-- https://w3id.org/italia/onto/Transparency/isPartOfObligation -->

    <owl:ObjectProperty rdf:about="https://w3id.org/italia/onto/Transparency/isPartOfObligation">
        <rdfs:domain rdf:resource="https://w3id.org/italia/onto/Transparency/TransparencyObligation"/>
        <rdfs:range rdf:resource="https://w3id.org/italia/onto/Transparency/TransparencyObligation"/>
        <rdfs:comment xml:lang="it">Questa proprietà lega un obbligo di trasparenza ad un obbligo di trasparenza più generale.</rdfs:comment>
        <rdfs:comment xml:lang="en">This property links a transparency obligation to a more general trasparency obligation.</rdfs:comment>
        <rdfs:isDefinedBy rdf:resource="https://w3id.org/italia/onto/Transparency"/>
        <rdfs:label xml:lang="en">part of transparency obligation</rdfs:label>
        <rdfs:label xml:lang="it">è parte di obbligo di trasparenza</rdfs:label>
    </owl:ObjectProperty>
    


    <!-- https://w3id.org/italia/onto/Transparency/isPerformedBy -->

    <owl:ObjectProperty rdf:about="https://w3id.org/italia/onto/Transparency/isPerformedBy">
        <rdfs:domain rdf:resource="https://w3id.org/italia/onto/Transparency/TransparencyActivity"/>
        <rdfs:range rdf:resource="https://w3id.org/italia/onto/l0/Agent"/>
        <rdfs:comment xml:lang="it">Questa proprietà lega una attività al soggetto che la esegue.</rdfs:comment>
        <rdfs:comment xml:lang="en">This property links a transparency activity to the agent that performs it.</rdfs:comment>
        <rdfs:isDefinedBy rdf:resource="https://w3id.org/italia/onto/Transparency"/>
        <rdfs:label xml:lang="en">is performed by</rdfs:label>
        <rdfs:label xml:lang="it">è eseguita da</rdfs:label>
    </owl:ObjectProperty>
    


    <!-- https://w3id.org/italia/onto/Transparency/mustBeUptodatedWithin -->

    <owl:ObjectProperty rdf:about="https://w3id.org/italia/onto/Transparency/mustBeUptodatedWithin">
        <rdfs:domain rdf:resource="https://w3id.org/italia/onto/Transparency/TransparencyResource"/>
        <rdfs:range rdf:resource="https://w3id.org/italia/onto/Transparency/UpdateFrequency"/>
        <rdfs:comment xml:lang="it">Questa proprietà collega una risorsa della trasparenza alla frequenza con cui deve addiornamento.</rdfs:comment>
        <rdfs:comment xml:lang="en">This property links a transparency resource to the prescribed update frequency.</rdfs:comment>
        <rdfs:isDefinedBy rdf:resource="https://w3id.org/italia/onto/Transparency"/>
        <rdfs:label xml:lang="it">deve essere aggiornato con</rdfs:label>
        <rdfs:label xml:lang="en">must be update within</rdfs:label>
    </owl:ObjectProperty>
    


    <!-- https://w3id.org/italia/onto/Transparency/obligedToEnforce -->

    <owl:ObjectProperty rdf:about="https://w3id.org/italia/onto/Transparency/obligedToEnforce">
        <rdfs:domain rdf:resource="https://w3id.org/italia/onto/COV/PublicOrganization"/>
        <rdfs:range rdf:resource="https://w3id.org/italia/onto/Transparency/TransparencyObligation"/>
        <rdfs:comment xml:lang="it">Questa proprietà lega una amministrazione pubblica gli obblighi di trasparenza che è obbligata a rispettare.</rdfs:comment>
        <rdfs:comment xml:lang="en">This property links a public organization to the transparecy obligations which is obliged to enforce.</rdfs:comment>
        <rdfs:isDefinedBy rdf:resource="https://w3id.org/italia/onto/Transparency"/>
        <rdfs:label xml:lang="it">obbligata a rispettare l&apos;obbligo</rdfs:label>
        <rdfs:label xml:lang="en">obliged to enforce obligation</rdfs:label>
    </owl:ObjectProperty>
    


    <!-- https://w3id.org/italia/onto/Transparency/performsTransparencyActivity -->

    <owl:ObjectProperty rdf:about="https://w3id.org/italia/onto/Transparency/performsTransparencyActivity">
        <rdfs:domain rdf:resource="https://w3id.org/italia/onto/l0/Agent"/>
        <rdfs:range rdf:resource="https://w3id.org/italia/onto/Transparency/TransparencyActivity"/>
        <rdfs:comment xml:lang="it">Questa proprietà lega una attività al soggetto che la esegue.</rdfs:comment>
        <rdfs:comment xml:lang="en">This property links a transparency activity to the agent that performs it.</rdfs:comment>
        <rdfs:isDefinedBy rdf:resource="https://w3id.org/italia/onto/Transparency"/>
        <rdfs:label xml:lang="it">esegue attività della trasparenza</rdfs:label>
        <rdfs:label xml:lang="en">performs transparency activity</rdfs:label>
    </owl:ObjectProperty>
    


    <!-- https://w3id.org/italia/onto/Transparency/previousVersionOf -->

    <owl:ObjectProperty rdf:about="https://w3id.org/italia/onto/Transparency/previousVersionOf">
        <rdfs:domain rdf:resource="https://w3id.org/italia/onto/Transparency/TransparencyResource"/>
        <rdfs:range rdf:resource="https://w3id.org/italia/onto/Transparency/TransparencyResource"/>
        <rdfs:comment xml:lang="it">Questa proprietà lega una risorsa alla sua versione successiva.</rdfs:comment>
        <rdfs:comment xml:lang="en">This property links a transparency resource to its next version.</rdfs:comment>
        <rdfs:isDefinedBy rdf:resource="https://w3id.org/italia/onto/Transparency"/>
        <rdfs:label xml:lang="en">previous version of</rdfs:label>
        <rdfs:label xml:lang="it">versione precedente di</rdfs:label>
    </owl:ObjectProperty>
    


    <!-- https://w3id.org/italia/onto/Transparency/refersToTransparencyEntity -->

    <owl:ObjectProperty rdf:about="https://w3id.org/italia/onto/Transparency/refersToTransparencyEntity">
        <rdfs:domain rdf:resource="https://w3id.org/italia/onto/Transparency/TransparencyResource"/>
        <rdfs:range>
            <owl:Class>
                <owl:unionOf rdf:parseType="Collection">
                    <rdf:Description rdf:about="https://w3id.org/italia/onto/l0/Activity"/>
                    <rdf:Description rdf:about="https://w3id.org/italia/onto/l0/Object"/>
                </owl:unionOf>
            </owl:Class>
        </rdfs:range>
        <rdfs:comment xml:lang="it">Questa proprità lega una risorsa della trasparenza alle entità ad essa collegata</rdfs:comment>
        <rdfs:comment xml:lang="en">This property links a transparency resource to the related entities.</rdfs:comment>
        <rdfs:isDefinedBy rdf:resource="https://w3id.org/italia/onto/Transparency"/>
        <rdfs:label xml:lang="en">refers to transparency entity</rdfs:label>
        <rdfs:label xml:lang="it">si riferisce a entità</rdfs:label>
    </owl:ObjectProperty>
    


    <!-- https://w3id.org/italia/onto/Transparency/refersToTransparencySubject -->

    <owl:ObjectProperty rdf:about="https://w3id.org/italia/onto/Transparency/refersToTransparencySubject">
        <rdfs:domain>
            <owl:Class>
                <owl:unionOf rdf:parseType="Collection">
                    <rdf:Description rdf:about="https://w3id.org/italia/onto/l0/Activity"/>
                    <rdf:Description rdf:about="https://w3id.org/italia/onto/l0/Object"/>
                </owl:unionOf>
            </owl:Class>
        </rdfs:domain>
        <rdfs:range rdf:resource="https://w3id.org/italia/onto/Transparency/TransparencySubject"/>
        <rdfs:comment xml:lang="it">Questa proprità lega una entità ai soggetti della trasparenza.</rdfs:comment>
        <rdfs:comment xml:lang="en">This property links an entity to the transparency subjects.</rdfs:comment>
        <rdfs:isDefinedBy rdf:resource="https://w3id.org/italia/onto/Transparency"/>
        <rdfs:label xml:lang="en">refers to transparency subject</rdfs:label>
        <rdfs:label xml:lang="it">si riferisce a soggetto</rdfs:label>
    </owl:ObjectProperty>
    


    <!-- https://w3id.org/italia/onto/Transparency/triggeredBy -->

    <owl:ObjectProperty rdf:about="https://w3id.org/italia/onto/Transparency/triggeredBy">
        <owl:inverseOf rdf:resource="https://w3id.org/italia/onto/Transparency/triggers"/>
        <rdfs:domain rdf:resource="https://w3id.org/italia/onto/Transparency/TransparencyActivity"/>
        <rdfs:range rdf:resource="https://w3id.org/italia/onto/Transparency/TransparencyObligation"/>
        <rdfs:comment xml:lang="it">Questa proprietà lega un obbligo di trasparenza all&apos;attività che attiva.</rdfs:comment>
        <rdfs:comment xml:lang="en">This property links a trasparency obbligation to the activty triggered by it.</rdfs:comment>
        <rdfs:isDefinedBy rdf:resource="https://w3id.org/italia/onto/Transparency"/>
        <rdfs:label xml:lang="it">attivato da</rdfs:label>
        <rdfs:label xml:lang="en">triggered by</rdfs:label>
    </owl:ObjectProperty>
    


    <!-- https://w3id.org/italia/onto/Transparency/triggers -->

    <owl:ObjectProperty rdf:about="https://w3id.org/italia/onto/Transparency/triggers">
        <rdfs:domain rdf:resource="https://w3id.org/italia/onto/Transparency/TransparencyObligation"/>
        <rdfs:range rdf:resource="https://w3id.org/italia/onto/Transparency/TransparencyActivity"/>
        <rdfs:comment xml:lang="it">Questa proprietà lega un obbligo di trasparenza all&apos;attività che attiva.</rdfs:comment>
        <rdfs:comment xml:lang="en">This property links a trasparency obbligation to the activty triggered by it.</rdfs:comment>
        <rdfs:isDefinedBy rdf:resource="https://w3id.org/italia/onto/Transparency"/>
        <rdfs:label xml:lang="it">attiva</rdfs:label>
        <rdfs:label xml:lang="en">triggers</rdfs:label>
    </owl:ObjectProperty>
    


    <!-- https://w3id.org/italia/onto/Transparency/updatedVersionOf -->

    <owl:ObjectProperty rdf:about="https://w3id.org/italia/onto/Transparency/updatedVersionOf">
        <rdfs:domain rdf:resource="https://w3id.org/italia/onto/Transparency/TransparencyResource"/>
        <rdfs:range rdf:resource="https://w3id.org/italia/onto/Transparency/TransparencyResource"/>
        <rdfs:comment xml:lang="it">Questa proprietà lega una risorsa alla sua versione precedente.</rdfs:comment>
        <rdfs:comment xml:lang="en">This property links a transparency resource to its previous version.</rdfs:comment>
        <rdfs:isDefinedBy rdf:resource="https://w3id.org/italia/onto/Transparency"/>
        <rdfs:label xml:lang="en">updated version of</rdfs:label>
        <rdfs:label xml:lang="it">versione aggiornata di</rdfs:label>
    </owl:ObjectProperty>
    


    <!-- 
    ///////////////////////////////////////////////////////////////////////////////////////
    //
    // Data properties
    //
    ///////////////////////////////////////////////////////////////////////////////////////
     -->

    


    <!-- https://w3id.org/italia/onto/SM/URL -->

    <rdf:Description rdf:about="https://w3id.org/italia/onto/SM/URL">
        <owl:equivalentProperty rdf:resource="https://w3id.org/italia/onto/Transparency/accessURL"/>
        <owl:equivalentProperty rdf:resource="https://w3id.org/italia/onto/Transparency/downloadURL"/>
    </rdf:Description>
    


    <!-- https://w3id.org/italia/onto/Transparency/accessURL -->

    <owl:DatatypeProperty rdf:about="https://w3id.org/italia/onto/Transparency/accessURL">
        <rdfs:domain rdf:resource="https://w3id.org/italia/onto/Transparency/TransparencyResource"/>
        <rdfs:range rdf:resource="http://www.w3.org/2001/XMLSchema#anyURI"/>
        <rdfs:comment xml:lang="it">Questa URL definisce l&apos;indirizzo di accesso e reperimento del contenuto informativo.</rdfs:comment>
        <rdfs:comment xml:lang="en">This URL defines the access address of the informative content.</rdfs:comment>
        <rdfs:isDefinedBy rdf:resource="https://w3id.org/italia/onto/Transparency"/>
        <rdfs:label xml:lang="it">URL di accesso alla risorsa</rdfs:label>
        <rdfs:label xml:lang="en">access URL</rdfs:label>
    </owl:DatatypeProperty>
    


    <!-- https://w3id.org/italia/onto/Transparency/downloadURL -->

    <owl:DatatypeProperty rdf:about="https://w3id.org/italia/onto/Transparency/downloadURL">
        <rdfs:domain rdf:resource="https://w3id.org/italia/onto/Transparency/TransparencyResource"/>
        <rdfs:range rdf:resource="http://www.w3.org/2001/XMLSchema#anyURI"/>
        <rdfs:comment xml:lang="it">Questa URL definisce l&apos;indirizzo di download del contenuto informativo.</rdfs:comment>
        <rdfs:comment xml:lang="en">This URL defines the download adress of the informative content.</rdfs:comment>
        <rdfs:isDefinedBy rdf:resource="https://w3id.org/italia/onto/Transparency"/>
        <rdfs:label xml:lang="it">URL di download del contenuto</rdfs:label>
        <rdfs:label xml:lang="en">download URL</rdfs:label>
    </owl:DatatypeProperty>
    


    <!-- https://w3id.org/italia/onto/Transparency/regulationReference -->

    <owl:DatatypeProperty rdf:about="https://w3id.org/italia/onto/Transparency/regulationReference">
        <rdfs:domain rdf:resource="https://w3id.org/italia/onto/Transparency/TransparencyObligation"/>
        <rdfs:range rdf:resource="http://www.w3.org/2000/01/rdf-schema#Literal"/>
        <rdfs:comment xml:lang="en">regulation referred to the transparency obligation.</rdfs:comment>
        <rdfs:comment xml:lang="it">riferimento normativo all&apos;obbligo di pubblicazione.</rdfs:comment>
        <rdfs:isDefinedBy rdf:resource="https://w3id.org/italia/onto/Transparency"/>
        <rdfs:label xml:lang="en">normative reference</rdfs:label>
        <rdfs:label xml:lang="it">riferimento normativo</rdfs:label>
    </owl:DatatypeProperty>
    


    <!-- 
    ///////////////////////////////////////////////////////////////////////////////////////
    //
    // Classes
    //
    ///////////////////////////////////////////////////////////////////////////////////////
     -->

    


    <!-- https://w3id.org/italia/onto/Transparency/Format -->

    <owl:Class rdf:about="https://w3id.org/italia/onto/Transparency/Format">
        <rdfs:subClassOf rdf:resource="https://w3id.org/italia/onto/l0/Characteristic"/>
        <rdfs:comment xml:lang="it">Questa classe indica il formato di una risorsa</rdfs:comment>
        <rdfs:comment xml:lang="en">This class represents the format of a resource.</rdfs:comment>
        <rdfs:isDefinedBy rdf:resource="https://w3id.org/italia/onto/Transparency"/>
        <rdfs:label xml:lang="en">Format</rdfs:label>
        <rdfs:label xml:lang="it">Formato</rdfs:label>
    </owl:Class>
    


    <!-- https://w3id.org/italia/onto/Transparency/TransparencyActivity -->

    <owl:Class rdf:about="https://w3id.org/italia/onto/Transparency/TransparencyActivity">
        <rdfs:subClassOf rdf:resource="https://w3id.org/italia/onto/l0/Activity"/>
        <rdfs:subClassOf>
            <owl:Restriction>
                <owl:onProperty rdf:resource="https://w3id.org/italia/onto/Transparency/generatesResource"/>
                <owl:someValuesFrom rdf:resource="https://w3id.org/italia/onto/Transparency/TransparencyResource"/>
            </owl:Restriction>
        </rdfs:subClassOf>
        <rdfs:subClassOf>
            <owl:Restriction>
                <owl:onProperty rdf:resource="https://w3id.org/italia/onto/Transparency/hasTransparencyActivityTypology"/>
                <owl:someValuesFrom rdf:resource="https://w3id.org/italia/onto/Transparency/TransparencyActivityTypology"/>
            </owl:Restriction>
        </rdfs:subClassOf>
        <rdfs:subClassOf>
            <owl:Restriction>
                <owl:onProperty rdf:resource="https://w3id.org/italia/onto/Transparency/isPerformedBy"/>
                <owl:qualifiedCardinality rdf:datatype="http://www.w3.org/2001/XMLSchema#nonNegativeInteger">1</owl:qualifiedCardinality>
                <owl:onClass rdf:resource="https://w3id.org/italia/onto/l0/Agent"/>
            </owl:Restriction>
        </rdfs:subClassOf>
        <rdfs:subClassOf>
            <owl:Restriction>
                <owl:onProperty rdf:resource="https://w3id.org/italia/onto/TI/date"/>
                <owl:qualifiedCardinality rdf:datatype="http://www.w3.org/2001/XMLSchema#nonNegativeInteger">1</owl:qualifiedCardinality>
                <owl:onDataRange>
                    <rdfs:Datatype>
                        <owl:unionOf rdf:parseType="Collection">
                            <rdf:Description rdf:about="http://www.w3.org/2001/XMLSchema#date"/>
                            <rdf:Description rdf:about="http://www.w3.org/2001/XMLSchema#dateTime"/>
                        </owl:unionOf>
                    </rdfs:Datatype>
                </owl:onDataRange>
            </owl:Restriction>
        </rdfs:subClassOf>
        <owl:disjointUnionOf rdf:parseType="Collection">
            <rdf:Description rdf:about="https://w3id.org/italia/onto/Transparency/TransparencyPublicationActivity"/>
            <rdf:Description rdf:about="https://w3id.org/italia/onto/Transparency/TransparencyUpdateActivity"/>
        </owl:disjointUnionOf>
        <rdfs:comment xml:lang="it">Questa classe rappresenta un&apos;attività di trasparenza come conseguenza di un obbligo di trasparenza.</rdfs:comment>
        <rdfs:comment xml:lang="en">This class represents a trasparency activity as an effect of a transparency obbligation. For example pubblication, update,...</rdfs:comment>
        <rdfs:isDefinedBy rdf:resource="https://w3id.org/italia/onto/Transparency"/>
        <rdfs:label xml:lang="it">Attività di trasparenza.</rdfs:label>
        <rdfs:label xml:lang="en">Transparency activity</rdfs:label>
    </owl:Class>
    


    <!-- https://w3id.org/italia/onto/Transparency/TransparencyActivityTypology -->

    <owl:Class rdf:about="https://w3id.org/italia/onto/Transparency/TransparencyActivityTypology">
        <rdfs:subClassOf rdf:resource="https://w3id.org/italia/onto/l0/Characteristic"/>
        <rdfs:comment xml:lang="it">Questa classe indica la tipologia di attività della trasparenza.</rdfs:comment>
        <rdfs:comment xml:lang="en">This class represents the transparency activity typology.</rdfs:comment>
        <rdfs:isDefinedBy rdf:resource="https://w3id.org/italia/onto/Transparency"/>
        <rdfs:label xml:lang="it">Tipologia di attività della trasparenza</rdfs:label>
        <rdfs:label xml:lang="en">Transparency activity typology</rdfs:label>
    </owl:Class>
    


    <!-- https://w3id.org/italia/onto/Transparency/TransparencyArchiveActivity -->

    <owl:Class rdf:about="https://w3id.org/italia/onto/Transparency/TransparencyArchiveActivity">
        <owl:equivalentClass>
            <owl:Restriction>
                <owl:onProperty rdf:resource="https://w3id.org/italia/onto/Transparency/hasTransparencyActivityTypology"/>
                <owl:hasValue rdf:resource="https://w3id.org/italia/onto/Transparency/TransparencyArchiveActivity"/>
            </owl:Restriction>
        </owl:equivalentClass>
        <rdfs:subClassOf rdf:resource="https://w3id.org/italia/onto/Transparency/TransparencyActivity"/>
        <owl:disjointWith rdf:resource="https://w3id.org/italia/onto/Transparency/TransparencyPublicationActivity"/>
    </owl:Class>
    


    <!-- https://w3id.org/italia/onto/Transparency/TransparencyDataTypology -->

    <owl:Class rdf:about="https://w3id.org/italia/onto/Transparency/TransparencyDataTypology">
        <rdfs:subClassOf rdf:resource="https://w3id.org/italia/onto/l0/Characteristic"/>
        <rdfs:comment xml:lang="it">Questa classe la tipologia di dati della trasparenza, nonchè la denominazione delle sotto-sezioni della sezione &apos;Amministrazione Trasparente&apos; del sito istituzionale delle pubbliche amministrazioni. Le voci sono controllate dal vocabolario &lt;https://w3id.org/italia/controlled-vocabulary/classifications-for-transparency/transparency-titulus&gt;.</rdfs:comment>
        <rdfs:comment xml:lang="en">This class represents typology of transaprecy data and moreover the subsections of the &apos;Transaprent Administrazion&apos; section of the official website of the public administrations. The individuals are controlled by the vocabulary &lt;https://w3id.org/italia/controlled-vocabulary/classifications-for-transparency/transparency-titulus&gt;.</rdfs:comment>
        <rdfs:isDefinedBy rdf:resource="https://w3id.org/italia/onto/Transparency"/>
        <rdfs:label xml:lang="it">Denominazione sotto-sezione Amministrazione Trasparente</rdfs:label>
        <rdfs:label xml:lang="it">Tipologia della trasparenza</rdfs:label>
        <rdfs:label xml:lang="en">Transparency data typology</rdfs:label>
        <rdfs:label xml:lang="en">Transparent administration sub-section denomination</rdfs:label>
        <l0:controlledVocabulary rdf:resource="https://w3id.org/italia/controlled-vocabulary/classifications-for-transparency/transparency-titulus"/>
    </owl:Class>
    


    <!-- https://w3id.org/italia/onto/Transparency/TransparencyObligation -->

    <owl:Class rdf:about="https://w3id.org/italia/onto/Transparency/TransparencyObligation">
        <rdfs:subClassOf rdf:resource="https://w3id.org/italia/onto/l0/Entity"/>
        <rdfs:subClassOf>
            <owl:Restriction>
                <owl:onProperty rdf:resource="https://w3id.org/italia/onto/Transparency/definesUpdateFrequency"/>
                <owl:someValuesFrom rdf:resource="https://w3id.org/italia/onto/Transparency/UpdateFrequency"/>
            </owl:Restriction>
        </rdfs:subClassOf>
        <rdfs:subClassOf>
            <owl:Restriction>
                <owl:onProperty rdf:resource="https://w3id.org/italia/onto/TI/atTime"/>
                <owl:allValuesFrom rdf:resource="https://w3id.org/italia/onto/TI/TimeInterval"/>
            </owl:Restriction>
        </rdfs:subClassOf>
        <rdfs:subClassOf>
            <owl:Restriction>
                <owl:onProperty rdf:resource="https://w3id.org/italia/onto/Transparency/regulationReference"/>
                <owl:someValuesFrom rdf:resource="http://www.w3.org/2000/01/rdf-schema#Literal"/>
            </owl:Restriction>
        </rdfs:subClassOf>
        <rdfs:subClassOf>
            <owl:Restriction>
                <owl:onProperty rdf:resource="https://w3id.org/italia/onto/l0/description"/>
                <owl:someValuesFrom rdf:resource="http://www.w3.org/2000/01/rdf-schema#Literal"/>
            </owl:Restriction>
        </rdfs:subClassOf>
        <rdfs:subClassOf>
            <owl:Restriction>
                <owl:onProperty rdf:resource="https://w3id.org/italia/onto/l0/name"/>
                <owl:someValuesFrom rdf:resource="http://www.w3.org/2000/01/rdf-schema#Literal"/>
            </owl:Restriction>
        </rdfs:subClassOf>
        <rdfs:comment xml:lang="it">Questa classe rappresenta gli argomenti oggetto di obbligo di pubblicazione per la normativa sulla trasparenza. Fa riferimento alla colonna &apos;denominazione obbligo&apos; dell&apos;allegato alla guida ANAC.</rdfs:comment>
        <rdfs:comment xml:lang="en">This class represents the topic object of transparency obligation according to the transparency normative. It&apos;s related to the &apos;denominazione obbligo&apos; column of the ANAC guideline attachment.</rdfs:comment>
        <rdfs:isDefinedBy rdf:resource="https://w3id.org/italia/onto/Transparency"/>
        <rdfs:label xml:lang="it">Obbligo di trasparenza</rdfs:label>
        <rdfs:label xml:lang="en">Obligation of transparency</rdfs:label>
    </owl:Class>
    


    <!-- https://w3id.org/italia/onto/Transparency/TransparencyObligationStatus -->

    <owl:Class rdf:about="https://w3id.org/italia/onto/Transparency/TransparencyObligationStatus">
        <rdfs:subClassOf rdf:resource="https://w3id.org/italia/onto/l0/Characteristic"/>
        <rdfs:comment xml:lang="it">Questa classe rappresenta lo stato dell&apos;obbligo di trasparenza. Per esempio vigente, decaduto,...</rdfs:comment>
        <rdfs:comment xml:lang="en">This class represents the transparency obbligation status. Ex: in force, deprecated,...</rdfs:comment>
        <rdfs:isDefinedBy rdf:resource="https://w3id.org/italia/onto/Transparency"/>
        <rdfs:label xml:lang="it">Stato dell&apos;obbligo di trasparenza.</rdfs:label>
        <rdfs:label xml:lang="en">Transparency obbligation status</rdfs:label>
    </owl:Class>
    


    <!-- https://w3id.org/italia/onto/Transparency/TransparencyPublicationActivity -->

    <owl:Class rdf:about="https://w3id.org/italia/onto/Transparency/TransparencyPublicationActivity">
        <owl:equivalentClass>
            <owl:Restriction>
                <owl:onProperty rdf:resource="https://w3id.org/italia/onto/Transparency/hasTransparencyActivityTypology"/>
                <owl:hasValue rdf:resource="https://w3id.org/italia/onto/Transparency/TransparencyPublicationActivity"/>
            </owl:Restriction>
        </owl:equivalentClass>
        <rdfs:subClassOf rdf:resource="https://w3id.org/italia/onto/Transparency/TransparencyActivity"/>
        <owl:disjointWith rdf:resource="https://w3id.org/italia/onto/Transparency/TransparencyUpdateActivity"/>
    </owl:Class>
    


    <!-- https://w3id.org/italia/onto/Transparency/TransparencyResource -->

    <owl:Class rdf:about="https://w3id.org/italia/onto/Transparency/TransparencyResource">
        <rdfs:subClassOf rdf:resource="https://w3id.org/italia/onto/l0/Object"/>
        <rdfs:subClassOf>
            <owl:Restriction>
                <owl:onProperty rdf:resource="https://w3id.org/italia/onto/Transparency/refersToTransparencyEntity"/>
                <owl:someValuesFrom>
                    <owl:Class>
                        <owl:unionOf rdf:parseType="Collection">
                            <rdf:Description rdf:about="https://w3id.org/italia/onto/l0/Activity"/>
                            <rdf:Description rdf:about="https://w3id.org/italia/onto/l0/Object"/>
                        </owl:unionOf>
                    </owl:Class>
                </owl:someValuesFrom>
            </owl:Restriction>
        </rdfs:subClassOf>
        <rdfs:subClassOf>
            <owl:Restriction>
                <owl:onProperty rdf:resource="https://w3id.org/italia/onto/l0/name"/>
                <owl:someValuesFrom rdf:resource="http://www.w3.org/2000/01/rdf-schema#Literal"/>
            </owl:Restriction>
        </rdfs:subClassOf>
        <rdfs:subClassOf>
            <owl:Restriction>
                <owl:onProperty rdf:resource="https://w3id.org/italia/onto/Transparency/accessURL"/>
                <owl:qualifiedCardinality rdf:datatype="http://www.w3.org/2001/XMLSchema#nonNegativeInteger">1</owl:qualifiedCardinality>
                <owl:onDataRange rdf:resource="http://www.w3.org/2001/XMLSchema#anyURI"/>
            </owl:Restriction>
        </rdfs:subClassOf>
        <rdfs:subClassOf>
            <owl:Restriction>
                <owl:onProperty rdf:resource="https://w3id.org/italia/onto/TI/modified"/>
                <owl:maxQualifiedCardinality rdf:datatype="http://www.w3.org/2001/XMLSchema#nonNegativeInteger">1</owl:maxQualifiedCardinality>
                <owl:onDataRange>
                    <rdfs:Datatype>
                        <owl:unionOf rdf:parseType="Collection">
                            <rdf:Description rdf:about="http://www.w3.org/2001/XMLSchema#date"/>
                            <rdf:Description rdf:about="http://www.w3.org/2001/XMLSchema#dateTime"/>
                            <rdf:Description rdf:about="http://www.w3.org/2001/XMLSchema#time"/>
                        </owl:unionOf>
                    </rdfs:Datatype>
                </owl:onDataRange>
            </owl:Restriction>
        </rdfs:subClassOf>
        <rdfs:comment xml:lang="it">Questa classe rappresenta i documenti, le informazioni e i dati oggetto di pubblicazione nei siti istituzionali delle pubbliche amministrazioni.</rdfs:comment>
        <rdfs:comment xml:lang="en">This class represents documents, informazions and data object of publication on the official website of the public administrations.</rdfs:comment>
        <rdfs:isDefinedBy rdf:resource="https://w3id.org/italia/onto/Transparency"/>
        <rdfs:label xml:lang="it">Risorsa di trasparenza</rdfs:label>
        <rdfs:label xml:lang="en">Transparency resource</rdfs:label>
    </owl:Class>
    


    <!-- https://w3id.org/italia/onto/Transparency/TransparencySubject -->

    <owl:Class rdf:about="https://w3id.org/italia/onto/Transparency/TransparencySubject">
        <rdfs:subClassOf rdf:resource="https://w3id.org/italia/onto/l0/Concept"/>
        <rdfs:subClassOf>
            <owl:Restriction>
                <owl:onProperty rdf:resource="https://w3id.org/italia/onto/l0/description"/>
                <owl:someValuesFrom rdf:resource="http://www.w3.org/2000/01/rdf-schema#Literal"/>
            </owl:Restriction>
        </rdfs:subClassOf>
        <rdfs:comment xml:lang="it">Questa classe rappresenta un soggetto (tema) collefato a un obbligo di trasparenza. Fa riferimento alla colonna &apos;contenuto dell&apos;obbligo&apos; dell&apos;allegato alla guida ANAC.</rdfs:comment>
        <rdfs:comment xml:lang="en">This class represents a subject releted to a transparency obbligation. It&apos;s related to the &apos;contenuto dell&apos;obbligo&apos; column of the ANAC guideline attachment.</rdfs:comment>
        <rdfs:isDefinedBy rdf:resource="https://w3id.org/italia/onto/Transparency"/>
        <rdfs:label xml:lang="it">Soggetto della trasparenza</rdfs:label>
        <rdfs:label xml:lang="en">Transparency subject</rdfs:label>
    </owl:Class>
    


    <!-- https://w3id.org/italia/onto/Transparency/TransparencyUpdateActivity -->

    <owl:Class rdf:about="https://w3id.org/italia/onto/Transparency/TransparencyUpdateActivity">
        <owl:equivalentClass>
            <owl:Restriction>
                <owl:onProperty rdf:resource="https://w3id.org/italia/onto/Transparency/hasTransparencyActivityTypology"/>
                <owl:hasValue rdf:resource="https://w3id.org/italia/onto/Transparency/TransparencyUpdateActivity"/>
            </owl:Restriction>
        </owl:equivalentClass>
        <rdfs:subClassOf rdf:resource="https://w3id.org/italia/onto/Transparency/TransparencyActivity"/>
    </owl:Class>
    


    <!-- https://w3id.org/italia/onto/Transparency/UpdateFrequency -->

    <owl:Class rdf:about="https://w3id.org/italia/onto/Transparency/UpdateFrequency">
        <rdfs:subClassOf rdf:resource="https://w3id.org/italia/onto/l0/Characteristic"/>
        <rdfs:comment xml:lang="it">Questa classe la frequenza di aggiornamento di una risorsa così come indicato dall&apos;obbligo ti trasaprenza.</rdfs:comment>
        <rdfs:comment xml:lang="en">This class represents the update frequency as prescribed by the transparency obbligation.</rdfs:comment>
        <rdfs:isDefinedBy rdf:resource="https://w3id.org/italia/onto/Transparency"/>
        <rdfs:label xml:lang="it">Frequenza di aggiornamento</rdfs:label>
        <rdfs:label xml:lang="en">Update frequency</rdfs:label>
    </owl:Class>
    


    <!-- https://w3id.org/italia/onto/l0/Activity -->

    <owl:Class rdf:about="https://w3id.org/italia/onto/l0/Activity"/>
    


    <!-- https://w3id.org/italia/onto/l0/Concept -->

    <owl:Class rdf:about="https://w3id.org/italia/onto/l0/Concept"/>
    


    <!-- 
    ///////////////////////////////////////////////////////////////////////////////////////
    //
    // Individuals
    //
    ///////////////////////////////////////////////////////////////////////////////////////
     -->

    


    <!-- http://spcdata.digitpa.gov.it/Amministrazione/agid -->

    <owl:NamedIndividual rdf:about="http://spcdata.digitpa.gov.it/Amministrazione/agid">
        <rdf:type rdf:resource="http://dati.gov.it/onto/dcatapit#Agent"/>
        <rdf:type rdf:resource="http://xmlns.com/foaf/0.1/Agent"/>
        <dct:identifier>agid</dct:identifier>
        <foaf:name xml:lang="it">Agenzia per l&apos;Italia Digitale</foaf:name>
        <foaf:name xml:lang="en">Italian Digital Agency</foaf:name>
    </owl:NamedIndividual>
    


    <!-- https://w3id.org/italia/data/distribution/TRAPIT-JSON-LD -->

    <owl:NamedIndividual rdf:about="https://w3id.org/italia/data/distribution/TRAPIT-JSON-LD">
        <rdf:type rdf:resource="https://w3id.org/italia/onto/ADMS/SemanticAssetDistribution"/>
        <dct:description xml:lang="it">Questa è la distribuzione JSON-LD dell&apos;ontologia dell&apos;amministrazione trasparente</dct:description>
        <dct:description xml:lang="en">This is the distribution in JSON-LD of the transparent administration</dct:description>
        <dct:format rdf:resource="http://publications.europa.eu/resource/authority/file-type/JSON_LD"/>
        <dct:license rdf:resource="https://w3id.org/italia/controlled-vocabulary/licences/A21_CCBY40"/>
        <dct:title xml:lang="it">Distribuzione JSON-LD ontologia Transparency-AP_IT</dct:title>
        <dct:title xml:lang="en">JSON-LD distribution of Transparency-AP_IT Ontology</dct:title>
        <dcat:accessURL rdf:resource="https://raw.githubusercontent.com/italia/daf-ontologie-vocabolari-controllati/master/Ontologie/Transparency/latest"/>
        <dcat:downloadURL rdf:resource="https://raw.githubusercontent.com/italia/daf-ontologie-vocabolari-controllati/master/Ontologie/Transparency/Transparency-AP_IT.jsonld"/>
    </owl:NamedIndividual>
    


    <!-- https://w3id.org/italia/data/distribution/TRAPIT-RDF-TURTLE -->

    <owl:NamedIndividual rdf:about="https://w3id.org/italia/data/distribution/TRAPIT-RDF-TURTLE">
        <rdf:type rdf:resource="https://w3id.org/italia/onto/ADMS/SemanticAssetDistribution"/>
        <dct:description xml:lang="it">Questa è la distribuzione RDF/Turtle dell&apos;ontologia dell&apos;amministrazione trasparente</dct:description>
        <dct:description xml:lang="en">This is the distribution in RDF/Turtle of the transparent administration</dct:description>
        <dct:format rdf:resource="http://publications.europa.eu/resource/authority/file-type/RDF_TURTLE"/>
        <dct:license rdf:resource="https://w3id.org/italia/controlled-vocabulary/licences/A21_CCBY40"/>
        <dct:title xml:lang="it">Distribuzione RDF/Turtle ontologia Transparency-AP_IT</dct:title>
        <dct:title xml:lang="en">RDF/Turtle distribution of Transparency-AP_IT Ontology</dct:title>
        <dcat:accessURL rdf:resource="https://raw.githubusercontent.com/italia/daf-ontologie-vocabolari-controllati/master/Ontologie/Transparency/latest"/>
        <dcat:downloadURL rdf:resource="https://raw.githubusercontent.com/italia/daf-ontologie-vocabolari-controllati/master/Ontologie/Transparency/Transparency-AP_IT.ttl"/>
    </owl:NamedIndividual>
    


    <!-- https://w3id.org/italia/data/distribution/TRAPIT-RDF-XML -->

    <owl:NamedIndividual rdf:about="https://w3id.org/italia/data/distribution/TRAPIT-RDF-XML">
        <rdf:type rdf:resource="https://w3id.org/italia/onto/ADMS/SemanticAssetDistribution"/>
        <dct:description xml:lang="it">Questa è la distribuzione RDF/XML dell&apos;ontologia dell&apos;amministrazione trasparente</dct:description>
        <dct:description xml:lang="en">This is the distribution in RDF/XML of the transparent administration</dct:description>
        <dct:format rdf:resource="http://publications.europa.eu/resource/authority/file-type/RDF_XML"/>
        <dct:license rdf:resource="https://w3id.org/italia/controlled-vocabulary/licences/A21_CCBY40"/>
        <dct:title xml:lang="it">Distribuzione RDF/XML ontologia Transparency-AP_IT</dct:title>
        <dct:title xml:lang="en">RDF/XML distribution of Transparency-AP_IT Ontology</dct:title>
        <dcat:accessURL rdf:resource="https://raw.githubusercontent.com/italia/daf-ontologie-vocabolari-controllati/master/Ontologie/Transparency/latest"/>
        <dcat:downloadURL rdf:resource="https://raw.githubusercontent.com/italia/daf-ontologie-vocabolari-controllati/master/Ontologie/Transparency/Transparency-AP_IT.rdf"/>
    </owl:NamedIndividual>
    


    <!-- https://w3id.org/italia/data/organization/private-organization/05481840964 -->

    <owl:NamedIndividual rdf:about="https://w3id.org/italia/data/organization/private-organization/05481840964">
        <rdf:type rdf:resource="http://dati.gov.it/onto/dcatapit#Agent"/>
        <rdf:type rdf:resource="http://xmlns.com/foaf/0.1/Agent"/>
        <dct:identifier>05481840964</dct:identifier>
        <foaf:name xml:lang="it">Almawave Srl</foaf:name>
    </owl:NamedIndividual>
    


    <!-- https://w3id.org/italia/onto/Transparency/Deprecated -->

    <owl:NamedIndividual rdf:about="https://w3id.org/italia/onto/Transparency/Deprecated">
        <rdf:type rdf:resource="https://w3id.org/italia/onto/Transparency/TransparencyObligationStatus"/>
        <l0:description xml:lang="it">Questo individuo rappresenta lo stato decaduto di un obbligo di trasparenza</l0:description>
        <l0:description xml:lang="en">This individual represents the status deprecated of a transparency obbligation</l0:description>
        <rdfs:isDefinedBy rdf:resource="https://w3id.org/italia/onto/Transparency"/>
        <rdfs:label xml:lang="it">decaduto</rdfs:label>
        <rdfs:label xml:lang="en">deprecated</rdfs:label>
    </owl:NamedIndividual>
    


    <!-- https://w3id.org/italia/onto/Transparency/InForce -->

    <owl:NamedIndividual rdf:about="https://w3id.org/italia/onto/Transparency/InForce">
        <rdf:type rdf:resource="https://w3id.org/italia/onto/Transparency/TransparencyObligationStatus"/>
        <l0:description xml:lang="it">Questo individuo rappresenta lo stato vigente di un obbligo di trasparenza</l0:description>
        <l0:description xml:lang="en">This individual represents the status in force of a transparency obbligation</l0:description>
        <rdfs:isDefinedBy rdf:resource="https://w3id.org/italia/onto/Transparency"/>
        <rdfs:label xml:lang="en">in force</rdfs:label>
        <rdfs:label xml:lang="it">vigente</rdfs:label>
    </owl:NamedIndividual>
    


    <!-- https://w3id.org/italia/onto/Transparency/TransparencyArchiveActivity -->

    <owl:NamedIndividual rdf:about="https://w3id.org/italia/onto/Transparency/TransparencyArchiveActivity">
        <rdf:type rdf:resource="https://w3id.org/italia/onto/Transparency/TransparencyActivityTypology"/>
        <l0:description xml:lang="it">Questo individuo rappresenta l&apos;attività di storicizzazione attivata da un obbligo di trasparenza.</l0:description>
        <l0:description xml:lang="en">This individual represents the archive activity triggered by a transparency obligation.</l0:description>
    </owl:NamedIndividual>
    


    <!-- https://w3id.org/italia/onto/Transparency/TransparencyPublicationActivity -->

    <owl:NamedIndividual rdf:about="https://w3id.org/italia/onto/Transparency/TransparencyPublicationActivity">
        <rdf:type rdf:resource="https://w3id.org/italia/onto/Transparency/TransparencyActivityTypology"/>
        <l0:description xml:lang="it">Questo individuo rappresenta l&apos;attività di pubblicazione attivata da un obbligo di trasparenza.</l0:description>
        <l0:description xml:lang="en">This individual represents the publication activity triggered by a transparency obligation.</l0:description>
    </owl:NamedIndividual>
    


    <!-- https://w3id.org/italia/onto/Transparency/TransparencyUpdateActivity -->

    <owl:NamedIndividual rdf:about="https://w3id.org/italia/onto/Transparency/TransparencyUpdateActivity">
        <rdf:type rdf:resource="https://w3id.org/italia/onto/Transparency/TransparencyActivityTypology"/>
        <l0:description xml:lang="it">Questo individuo rappresenta l&apos;attività di aggiornamento attivata da un obbligo di trasparenza.</l0:description>
        <l0:description xml:lang="en">This individual represents the update activity triggered by a transparency obligation.</l0:description>
    </owl:NamedIndividual>
    


    <!-- 
    ///////////////////////////////////////////////////////////////////////////////////////
    //
    // Annotations
    //
    ///////////////////////////////////////////////////////////////////////////////////////
     -->

    <rdf:Description rdf:about="https://w3id.org/italia/onto/Transparency/TransparencyArchiveActivity">
        <rdfs:comment xml:lang="en">This class represents an archive activity as an effect of a transparency obbligation.</rdfs:comment>
        <rdfs:label xml:lang="it">storicizzazione</rdfs:label>
        <rdfs:isDefinedBy rdf:resource="https://w3id.org/italia/onto/Transparency"/>
        <rdfs:comment xml:lang="it">Questa classe rappresenta un&apos;attività di storicizzazione come conseguenza di un obbligo di trasparenza.</rdfs:comment>
        <rdfs:label xml:lang="it">archive</rdfs:label>
        <rdfs:label xml:lang="it">Attività di trasparenza: Storicizzazione.</rdfs:label>
        <rdfs:label xml:lang="en">Transparency activity: Archive.</rdfs:label>
    </rdf:Description>
    <rdf:Description rdf:about="https://w3id.org/italia/onto/Transparency/TransparencyPublicationActivity">
        <rdfs:comment xml:lang="it">Questa classe rappresenta un&apos;attività di pubblicazione come conseguenza di un obbligo di trasparenza.</rdfs:comment>
        <rdfs:isDefinedBy rdf:resource="https://w3id.org/italia/onto/Transparency"/>
        <rdfs:label xml:lang="it">Attività di trasparenza: Pubblicazione.</rdfs:label>
        <rdfs:label xml:lang="it">publication</rdfs:label>
        <rdfs:label xml:lang="en">Transparency activity: Publication.</rdfs:label>
        <rdfs:label xml:lang="en">Transparency activity: Publication</rdfs:label>
        <rdfs:comment xml:lang="en">This class represents a publication activity as an effect of a transparency obbligation.</rdfs:comment>
        <rdfs:label xml:lang="it">pubblicazione</rdfs:label>
    </rdf:Description>
    <rdf:Description rdf:about="https://w3id.org/italia/onto/Transparency/TransparencyUpdateActivity">
        <rdfs:isDefinedBy rdf:resource="https://w3id.org/italia/onto/Transparency"/>
        <rdfs:label xml:lang="it">aggiornamento</rdfs:label>
        <rdfs:label xml:lang="it">Attività di trasparenza: Aggiornamento.</rdfs:label>
        <rdfs:label xml:lang="en">Transparency activity: Update.</rdfs:label>
        <rdfs:label xml:lang="it">update</rdfs:label>
        <rdfs:comment xml:lang="it">Questa classe rappresenta un&apos;attività di aggiornamento come conseguenza di un obbligo di trasparenza.</rdfs:comment>
        <rdfs:comment xml:lang="en">This class represents an update activity as an effect of a transparency obbligation.</rdfs:comment>
    </rdf:Description>
</rdf:RDF>



<!-- Generated by the OWL API (version 4.5.9.2019-02-01T07:24:44Z) https://github.com/owlcs/owlapi -->

